made type for monomials

thys/Polynomials/Polynomials.thy
@@ -25,6 +25,8 @@ with IsaFoR/CeTA. If not, see <http://www.gnu.org/licenses/>.
 
 section {* Polynomials *}
 
+(* TODO: attempt to turn polynomials into type *)
+
 theory Polynomials
 imports 
   "Abstract-Rewriting.SN_Orders"
@@ -38,19 +40,11 @@ datatype (vars_tpoly: 'v, nums_tpoly: 'a)tpoly = PVar 'v | PNum 'a | PSum "('v,'
 
 type_synonym ('v,'a)assign = "'v \<Rightarrow> 'a"
 
-fun eval_tpoly :: "('v,'a::{zero,one,plus,times})assign \<Rightarrow> ('v,'a)tpoly \<Rightarrow> 'a"
+primrec eval_tpoly :: "('v,'a::{monoid_add,monoid_mult})assign \<Rightarrow> ('v,'a)tpoly \<Rightarrow> 'a"
 where "eval_tpoly \<alpha> (PVar x) = \<alpha> x"
    |  "eval_tpoly \<alpha> (PNum a) = a"
-   |  "eval_tpoly \<alpha> (PSum []) = 0"
-   |  "eval_tpoly \<alpha> (PSum (p # ps)) = eval_tpoly \<alpha> p + eval_tpoly \<alpha> (PSum ps)"
-   |  "eval_tpoly \<alpha> (PMult []) = 1"
-   |  "eval_tpoly \<alpha> (PMult (p # ps)) = eval_tpoly \<alpha> p * eval_tpoly \<alpha> (PMult ps)"
-
-lemma eval_tpoly_PSum: "eval_tpoly A (PSum ps) = sum_list (map (eval_tpoly A) ps)"
-  by (induct ps) auto
-
-lemma eval_tpoly_PMult: "eval_tpoly A (PMult ps) = prod_list (map (eval_tpoly A) ps)"
-  by (induct ps) auto
+   |  "eval_tpoly \<alpha> (PSum ps) = sum_list (map (eval_tpoly \<alpha>) ps)"
+   |  "eval_tpoly \<alpha> (PMult ps) = prod_list (map (eval_tpoly \<alpha>) ps)"
 
 subsection {* Polynomials represented in normal form as lists of monomials *}
 text {*
@@ -61,7 +55,7 @@ text {*
 text {* Definition of type @{text monom} *}
 
 
-type_synonym 'v monom = "('v \<times> nat)list" 
+type_synonym 'v monom_list = "('v \<times> nat)list" 
 text {* 
 \begin{itemize}
 \item $[(x,n),(y,m)]$ represent $x^n \cdot y^m$
@@ -71,56 +65,42 @@ text {*
 \end{itemize}
 *}
 
-definition monom_inv :: "'v monom \<Rightarrow> bool"
-where "monom_inv m \<equiv> (\<forall> (x,n) \<in> set m. 1 \<le> n) \<and> distinct (map fst m)"
+context linorder
+begin
+definition monom_inv :: "'a monom_list \<Rightarrow> bool" where 
+  "monom_inv m \<equiv> (\<forall> (x,n) \<in> set m. 1 \<le> n) \<and> distinct (map fst m) \<and> sorted (map fst m)"
 
+fun eval_monom_list :: "('a,'b :: comm_semiring_1)assign \<Rightarrow> ('a monom_list) \<Rightarrow> 'b" where 
+  "eval_monom_list \<alpha> [] = 1"
+| "eval_monom_list \<alpha> ((x,p) # m) = eval_monom_list \<alpha> m * (\<alpha> x)^p"
 
-fun eval_monom :: "('v,'a :: comm_semiring_1)assign \<Rightarrow> ('v monom) \<Rightarrow> 'a"
-where "eval_monom \<alpha> [] = 1"
-   |  "eval_monom \<alpha> ((x,p) # m) = eval_monom \<alpha> m * (\<alpha> x)^p"
-
-lemma eval_monom_list[simp]: "eval_monom \<alpha> (m @ n) = eval_monom \<alpha> m * eval_monom \<alpha> n"
+lemma eval_monom_list[simp]: "eval_monom_list \<alpha> (m @ n) = eval_monom_list \<alpha> m * eval_monom_list \<alpha> n"
   by (induct m, auto simp: field_simps)
 
-
-text {*
-equality of monomials should be able to identify $x^2 \cdot y$ with $y \cdot x^2$,
-essentially, it checks for permutations. Checking of permutations 
-suffices, since in $x^2 \cdot x^1 = x^3$, the left-hand side should not
-be constructed due to the invariant, that every variable occurs at
-most once in a monomial.
-*}
-fun eq_monom :: "'v monom \<Rightarrow> 'v monom \<Rightarrow> bool" (infix "=m" 51) where
-  "[] =m n = (n = [])" 
-| "(x,p) # m =m n =
-  (case List.extract (\<lambda>yq. fst yq = x) n of
-    None \<Rightarrow> False
-  | Some (n1,(_,q),n2) \<Rightarrow> p = q \<and> m =m (n1 @ n2))"
-
-lemma eq_monom_refl: "m =m m"
-proof (induct m)
-  case (Cons xp m)
-  show ?case 
-  proof (cases xp)
-    case (Pair x p)
-    show ?thesis
-      by (simp add: Pair Cons extract_Cons_code)
-  qed
-qed simp
-
-definition sum_var_list :: "'v monom \<Rightarrow> 'v \<Rightarrow> nat"
-where "sum_var_list m x \<equiv> sum_list (map (\<lambda> (y,c). if x = y then c else 0) m)"
+definition sum_var_list :: "'a monom_list \<Rightarrow> 'a \<Rightarrow> nat" where
+  "sum_var_list m x \<equiv> sum_list (map (\<lambda> (y,c). if x = y then c else 0) m)"
 
 lemma sum_var_list_not: "x \<notin> fst ` set m \<Longrightarrow> sum_var_list m x = 0"
-unfolding sum_var_list_def
-  by (induct m, auto)
+  unfolding sum_var_list_def by (induct m, auto)
 
 text {*
 show that equality of monomials is equivalent to statement that 
 all variables occur with the same (accumulated) power;
 afterwards properties like transitivity, etc. are easy to prove *}
+
+lemma monom_inv_Cons: assumes "monom_inv ((x,p) # m)" 
+  and "y \<le> x" shows "y \<notin> fst ` set m" 
+proof -
+  define M where "M = map fst m" 
+  from assms[unfolded monom_inv_def] 
+  have "distinct (x # map fst m)" "sorted (x # map fst m)"  by auto
+  with assms(2) have "y \<notin> set (map fst m)" unfolding M_def[symmetric]
+    by (induct M, auto simp: sorted_Cons)
+  thus ?thesis by auto
+qed
+
 lemma eq_monom_sum_var_list: assumes "monom_inv m" and "monom_inv n"
-  shows "eq_monom m n = (\<forall> x. sum_var_list m x = sum_var_list n x)" (is "?l = ?r")
+  shows "(m = n) = (\<forall> x. sum_var_list m x = sum_var_list n x)" (is "?l = ?r")
 using assms
 proof (induct m arbitrary: n)
   case Nil
@@ -134,87 +114,52 @@ proof (induct m arbitrary: n)
 next
   case (Cons xp m)
   obtain x p where xp: "xp = (x,p)" by (cases xp, auto)
-  with Cons(2) have p: "0 < p" and x: "x \<notin> fst ` set m" and m: "monom_inv m" unfolding monom_inv_def by auto
+  with Cons(2) have p: "0 < p" and x: "x \<notin> fst ` set m" and m: "monom_inv m" unfolding monom_inv_def 
+    by (auto simp: sorted_Cons)
   show ?case 
-  proof (cases "List.extract (\<lambda> yq. fst yq = x) n")
-    case None
-    hence not1: "x \<notin> fst ` set n" by (auto simp: extract_None_iff)
-    show ?thesis
-      by (simp add: xp Cons None, rule exI[of _ x], simp add: sum_var_list_not[OF not1], simp add: sum_var_list_def p)
+  proof (cases n)
+    case Nil
+    thus ?thesis by (auto simp: xp sum_var_list_def p intro!: exI[of _ x])
   next
-    case (Some res)
-    obtain n1 yq n2 where "res = (n1,yq,n2)" by (cases res, auto)
-    then obtain y q where "res = (n1,(y,q),n2)" by (cases yq, auto)
-    with extract_SomeE[OF Some[simplified this]] have n: "n = n1 @ (x,q) # n2" and res: "res = (n1,(x,q),n2)"  by auto
-    from Cons(3)[unfolded n] have q: "1 \<le> q" and n1n2: "x \<notin> fst ` (set (n1 @ n2))" and n1n2m: "monom_inv (n1 @ n2)" unfolding  monom_inv_def by auto
-    show ?thesis 
-    proof (cases "p = q")
-      case False
-      have "sum_var_list ((x,p) # m) x = p + sum_var_list m x" unfolding sum_var_list_def by auto
-      also have "\<dots> = p" using sum_var_list_not[OF x] by simp
-      also have "\<dots> \<noteq> q" using False .
-      also have "q = q + sum_var_list (n1 @ n2) x" using sum_var_list_not[OF n1n2] by simp
-      also have "\<dots> = sum_var_list n x" unfolding n sum_var_list_def by auto
-      finally have not2: "sum_var_list ((x,p) # m) x \<noteq> sum_var_list n x" . 
-      show ?thesis
-        by (simp add: xp Some res False, rule exI[of _ x], rule not2)
+    case n: (Cons yq n')
+    from Cons(3)[unfolded n] have n': "monom_inv n'" by (auto simp: monom_inv_def sorted_Cons)
+    show ?thesis
+    proof (cases "yq = xp")
+      case True
+      show ?thesis unfolding n True using Cons(1)[OF m n'] by (auto simp: xp sum_var_list_def)
     next
-      case True 
-      {
-        fix y
-        have "(sum_var_list m y = sum_var_list (n1 @ n2) y) =
-          (sum_var_list ((x,q) # m) y = sum_var_list (n1 @ (x,q) # n2) y)"
-          by (unfold sum_var_list_def, cases "x = y", auto)
-      }
-      hence id: "(\<forall> y. sum_var_list m y = sum_var_list (n1 @ n2) y) = 
-          (\<forall> y. sum_var_list ((x,q) # m) y = sum_var_list (n1 @ (x,q) # n2) y)"
-        by blast
-      show ?thesis 
-        by (simp add: xp Some res True Cons(1)[OF m n1n2m], simp only: n, rule id)
+      case False
+      obtain y q where yq: "yq = (y,q)" by force
+      from Cons(3)[unfolded n yq monom_inv_def] have q: "q > 0" by auto
+      define z where "z = min x y" 
+      have zm: "z \<notin> fst ` set m" using Cons(2) unfolding xp z_def
+        by (rule monom_inv_Cons, simp)
+      have zn': "z \<notin> fst ` set n'" using Cons(3) unfolding n yq z_def
+        by (rule monom_inv_Cons, simp)
+      have smz: "sum_var_list (xp # m) z = sum_var_list [(x,p)] z" 
+        using sum_var_list_not[OF zm] by (simp add: sum_var_list_def xp)
+      also have "\<dots> \<noteq> sum_var_list [(y,q)] z" using False unfolding xp yq 
+        by (auto simp: sum_var_list_def z_def p q min_def)
+      also have "sum_var_list [(y,q)] z = sum_var_list n z" 
+        using sum_var_list_not[OF zn'] by (simp add: sum_var_list_def n yq)
+      finally show ?thesis using False unfolding n by auto
     qed
   qed
 qed
-      
-
-lemma eq_monom_sym: assumes m: "monom_inv m" and n: "monom_inv n" shows "(m =m n) = (n =m m)"
-  by (simp add: eq_monom_sum_var_list[OF m n] eq_monom_sum_var_list[OF n m] sum_var_list_def, auto)
-
-lemma eq_monom_trans: assumes m1: "monom_inv m1" and m2: "monom_inv m2" and m3: "monom_inv m3" shows 
-  "m1 =m m2 \<Longrightarrow> m2 =m m3 \<Longrightarrow> m1 =m m3"
-  by (simp add: eq_monom_sum_var_list[OF m1 m2] eq_monom_sum_var_list[OF m2 m3] eq_monom_sum_var_list[OF m1 m3] sum_var_list_def)
-
-text {*
-show that equality of monomials implies equal evaluations *}    
-lemma eq_monom: "m =m n \<Longrightarrow> eval_monom \<alpha> m = eval_monom \<alpha> n"
-proof (induct m arbitrary: n)
-  case (Cons xp m) note mCons = this
-  show ?case
-  proof (cases xp)
-    case (Pair x p)
-    show ?thesis 
-    proof (cases "List.extract (\<lambda> yq. fst yq = x) n")
-      case None
-      with Cons Pair show ?thesis by auto
-    next
-      case (Some res)
-      obtain n1 yq n2 where "res = (n1,yq,n2)" by (cases res, auto)
-      then obtain y q where res: "res = (n1,(y,q),n2)" by (cases yq, auto)
-      from extract_SomeE[OF Some[simplified res]] mCons(2)  Some Pair res have n: "n = n1 @ (x,p) # n2" and rec: "m =m (n1 @ n2)" by auto
-      show ?thesis by (simp add: Pair mCons(1)[OF rec] n field_simps)
-    qed
-  qed
-qed simp
 
 text {*
   equality of monomials is also a complete for several carriers, e.g. the naturals, integers, where $x^p = x^q$ implies $p = q$.
   note that it is not complete for carriers like the Booleans where e.g. $x^{Suc(m)} = x^{Suc(n)}$ for all $n,m$.
 *}
+(*
 lemma eq_monom_inv: 
-  fixes m :: "'v monom"
-  assumes exp_inject: "\<And> p q :: nat. \<exists> base :: 'a :: poly_carrier. base^p = base^q \<Longrightarrow> p = q" and m: "monom_inv m" and n: "monom_inv n" shows "(m =m n) = (\<forall> \<alpha> :: ('v,'a :: poly_carrier)assign. eval_monom \<alpha> m = eval_monom \<alpha> n)"
-proof(intro iffI allI, rule eq_monom)
-  assume "\<forall> \<alpha> :: ('v,'a :: poly_carrier)assign. eval_monom \<alpha> m = eval_monom \<alpha> n"
-  with m n show "m =m n"
+  fixes m :: "'v :: linorder monom_list"
+  assumes exp_inject: "\<And> p q :: nat. \<exists> base :: 'a :: poly_carrier. base^p = base^q \<Longrightarrow> p = q" 
+  and m: "monom_inv m" and n: "monom_inv n" 
+  shows "(m = n) = (\<forall> \<alpha> :: ('v,'a :: poly_carrier)assign. eval_monom_list \<alpha> m = eval_monom_list \<alpha> n)"
+proof(intro iffI allI, rule eq_monom_list)
+  assume "\<forall> \<alpha> :: ('v,'a :: poly_carrier)assign. eval_monom_list \<alpha> m = eval_monom_list \<alpha> n"
+  with m n show "m = n"
   proof (induct m arbitrary: n)
     case Nil
     show ?case 
@@ -222,7 +167,7 @@ proof(intro iffI allI, rule eq_monom)
       case (Cons yq nn)
       with Nil obtain y q where yq: "yq = (y,q)" and "1 \<le> q" by (cases yq, auto simp: monom_inv_def)
       then obtain qq where q: "q = Suc (qq)" by (cases q, auto)
-      from Nil(3) have "1 = eval_monom (\<lambda> x. 0 :: 'a) n" (is "?one = _") by simp
+      from Nil(3) have "1 = eval_monom_list (\<lambda> x. 0 :: 'a) n" (is "?one = _") by simp
       also have "\<dots> = 0" by (simp add: Cons yq q)
       finally show ?thesis by simp
     qed simp
@@ -233,9 +178,9 @@ proof(intro iffI allI, rule eq_monom)
       case (Pair x p)
       let ?ass = "(\<lambda> v y. if x = y then v else 1 :: 'a)"
       {
-        fix v :: 'a and m :: "'v monom"
+        fix v :: 'a and m :: "'v monom_list"
         assume "x \<notin> fst ` (set m)"
-        hence "eval_monom (?ass v) m = 1"
+        hence "eval_monom_list (?ass v) m = 1"
         proof (induct m)
           case (Cons yp m)
           thus ?case 
@@ -243,12 +188,12 @@ proof(intro iffI allI, rule eq_monom)
         qed simp
       } note ass = this
       from Cons(2)[unfolded Pair] obtain pp where p: "p = Suc pp" and xm: "x \<notin> fst ` (set m)" unfolding monom_inv_def by (cases p, auto)
-      from ass[OF xm] have "\<And> v. eval_monom (?ass v) (xp # m) = v * v^pp" by (simp add: Pair p)
-      with Cons(4) have eval: "\<And> v. eval_monom (?ass v) n = v * v^pp" by auto
+      from ass[OF xm] have "\<And> v. eval_monom_list (?ass v) (xp # m) = v * v^pp" by (simp add: Pair p)
+      with Cons(4) have eval: "\<And> v. eval_monom_list (?ass v) n = v * v^pp" by auto
       show ?thesis 
       proof (cases "List.extract (\<lambda> yq. fst yq = x) n")
         case None
-        with ass[of n] have "\<And> v. eval_monom (?ass v) n = 1" by (auto simp: extract_None_iff)
+        with ass[of n] have "\<And> v. eval_monom_list (?ass v) n = 1" by (auto simp: extract_None_iff)
         from this[of 0] eval[of 0] show ?thesis by simp
       next
         case (Some res)
@@ -256,29 +201,29 @@ proof(intro iffI allI, rule eq_monom)
         then obtain y q where "res = (n1,(y,q),n2)" by (cases yq, auto)        
         from extract_SomeE[OF Some[simplified this]] mCons(2)  Some Pair this have n: "n = n1 @ (x,q) # n2" and res: "res = (n1,(x,q),n2)" by auto
         from mCons(3)[unfolded n] have xn: "x \<notin> fst ` (set (n1 @ n2))" unfolding monom_inv_def by auto
-        have "\<And> v. eval_monom (?ass v) n = v^q * eval_monom (?ass v) (n1 @ n2)" unfolding n by (auto simp: field_simps)
+        have "\<And> v. eval_monom_list (?ass v) n = v^q * eval_monom_list  (?ass v) (n1 @ n2)" unfolding n by (auto simp: field_simps)
         from eval[unfolded this ass[OF xn]] have id: "\<And> v :: 'a. v^p = v^q" using p by auto
         from exp_inject[of p q] id have pq: "p = q" by auto
         have rec: "((xp # m) =m n) = (m =m (n1 @ n2))" by (simp add: Pair Some res pq)
-        have ass: "\<forall>\<alpha> :: ('v,'a)assign. eval_monom \<alpha> m = eval_monom \<alpha> (n1 @ n2)"
+        have ass: "\<forall>\<alpha> :: ('v,'a)assign. eval_monom_list  \<alpha> m = eval_monom_list \<alpha> (n1 @ n2)"
         proof
           fix \<alpha> :: "('v,'a)assign"
-          show "eval_monom \<alpha> m = eval_monom \<alpha> (n1 @ n2)"
+          show "eval_monom_list \<alpha> m = eval_monom_list \<alpha> (n1 @ n2)"
           proof (rule ccontr)
             assume neq: "\<not> ?thesis"
             let ?ass =  "\<lambda> y :: 'v. if x = y then 1 :: 'a else \<alpha> y"
             {
-              fix m :: "'v monom"
+              fix m :: "'v monom_list"
               assume "x \<notin> fst ` set m"
-              hence "eval_monom \<alpha> m = eval_monom ?ass m"
+              hence "eval_monom_list \<alpha> m = eval_monom_list ?ass m"
                 by (induct m, auto)
             } note ass = this
-            have "eval_monom \<alpha> (n1 @ n2) = eval_monom ?ass (n1 @ n2)" using ass[OF xn] .
-            also have "\<dots> = eval_monom ?ass n" unfolding n by auto
-            also have "\<dots> = eval_monom ?ass ((xp # m))" using mCons(4) by auto
-            also have "\<dots> = eval_monom ?ass m" unfolding Pair by simp
-            also have "\<dots> = eval_monom \<alpha> m" using ass[OF xm] by simp 
-            also have "\<dots> \<noteq> eval_monom \<alpha> (n1 @ n2)" by (rule neq)
+            have "eval_monom_list \<alpha> (n1 @ n2) = eval_monom_list ?ass (n1 @ n2)" using ass[OF xn] .
+            also have "\<dots> = eval_monom_list ?ass n" unfolding n by auto
+            also have "\<dots> = eval_monom_list ?ass ((xp # m))" using mCons(4) by auto
+            also have "\<dots> = eval_monom_list ?ass m" unfolding Pair by simp
+            also have "\<dots> = eval_monom_list \<alpha> m" using ass[OF xm] by simp 
+            also have "\<dots> \<noteq> eval_monom_list \<alpha> (n1 @ n2)" by (rule neq)
             finally show False by simp
           qed
         qed
@@ -287,127 +232,162 @@ proof(intro iffI allI, rule eq_monom)
       qed
     qed    
   qed
-qed simp  
+qed simp  *)
 
-declare eq_monom.simps[simp del]
+abbreviation (input) monom_list_vars :: "'a monom_list \<Rightarrow> 'a set"
+  where "monom_list_vars m \<equiv> fst ` set m"
 
-abbreviation monom_vars :: "'v monom \<Rightarrow> 'v set"
-  where "monom_vars m \<equiv> fst ` set m"
+fun monom_mult_list :: "'a monom_list \<Rightarrow> 'a monom_list \<Rightarrow> 'a monom_list" where 
+  "monom_mult_list [] n = n"
+| "monom_mult_list ((x,p) # m) n = (case n of
+     Nil \<Rightarrow> (x,p) # m 
+   | (y,q) # n' \<Rightarrow> if x = y then (x,p + q) # monom_mult_list m n' else
+       if x < y then (x,p) # monom_mult_list m n else (y,q) # monom_mult_list ((x,p) # m) n')"
 
-fun monom_mult :: "'v monom \<Rightarrow> 'v monom \<Rightarrow> 'v monom"
-where "monom_mult [] n = n"
-  |   "monom_mult ((x,p) # m) n = (case List.extract (\<lambda> yq. fst yq = x) n of
-                           None \<Rightarrow> (x,p) # monom_mult m n 
-                         | Some (n1,(_,q),n2) \<Rightarrow> (x,p+q) # monom_mult m (n1 @ n2))"
+lemma monom_list_mult_list_vars: "monom_list_vars (monom_mult_list m1 m2) = monom_list_vars m1 \<union> monom_list_vars m2"
+  by (induct m1 m2 rule: monom_mult_list.induct, auto split: list.splits)
 
-lemma monom_mult_vars: "monom_vars (monom_mult m1 m2) = monom_vars m1 \<union> monom_vars m2"
-proof (induct m1 arbitrary: m2)
-  case (Cons xp m) note mCons = this
+
+lemma monom_mult_list_inv: "monom_inv m1 \<Longrightarrow> monom_inv m2 \<Longrightarrow> monom_inv (monom_mult_list m1 m2)"
+proof (induct m1 m2 rule: monom_mult_list.induct)
+  case (2 x p m n')
+  note IH = 2(1-3)
+  note xpm = 2(4)
+  note n' = 2(5)
   show ?case
-  proof (cases xp)
-    case (Pair x p)
-    show ?thesis 
-    proof (cases "List.extract (\<lambda> yq. fst yq = x) m2")
-      case None
-      with Cons Pair show ?thesis by auto 
-    next
-      case (Some res)
-      obtain n1 yq n2 where "res = (n1,yq,n2)" by (cases res, auto)
-      then obtain y q where res: "res = (n1,(y,q),n2)" by (cases yq, auto)
-      from extract_SomeE[OF Some[simplified res]] Some Pair res have m2: "m2 = n1 @ (x,q) # n2"
-        and rec: "monom_mult (xp # m) m2 = (x, p+q) # monom_mult m (n1 @ n2)" by auto
-      show ?thesis by (simp only: rec, simp add: mCons Pair m2)
-    qed
-  qed
-qed simp
-
-
-lemma monom_mult_inv: "monom_inv m1 \<Longrightarrow> monom_inv m2 \<Longrightarrow> monom_inv (monom_mult m1 m2)"
-proof (induct m1 arbitrary: m2)
-  case Nil thus ?case by (simp add: monom_inv_def)
-next
-  case (Cons xp m1)
-  obtain x p where xp: "xp = (x,p)" by (cases xp) auto
-  from xp Cons(2) have m1: "monom_inv m1" and x: "x \<notin> monom_vars m1" and p: "1 \<le> p" by (auto simp: monom_inv_def)
-  show ?case 
-  proof (cases "List.extract (\<lambda> yq. fst yq = x) m2")
-    case None
-    hence "x \<notin> monom_vars m2" by (auto simp: extract_None_iff)
-    from x this have x: "x \<notin> monom_vars (monom_mult m1 m2)" by (simp add: monom_mult_vars)
-    with None Cons(1)[OF m1 Cons(3)] x p xp show ?thesis by (auto simp: monom_inv_def)
+  proof (cases n')
+    case Nil
+    with xpm show ?thesis by auto
   next
-    case (Some res)
-    obtain n1 yq n2 where "res = (n1,yq,n2)" by (cases res, auto)
-    then obtain y q where res: "res = (n1,(y,q),n2)" by (cases yq, auto)
-    from extract_SomeE[OF Some[simplified res]] Some xp res have m2: "m2 = n1 @ (x,q) # n2"
-      and rec: "monom_mult (xp # m1) m2 = (x, p+q) # monom_mult m1 (n1 @ n2)" by auto
-    from Cons(3) m2 have xn1: "x \<notin> monom_vars (n1 @ n2)"
-      and n1n2: "monom_inv (n1 @ n2)" and q: "1 \<le> q" by (auto simp: monom_inv_def)
-    from x xn1 have x: "x \<notin> monom_vars (monom_mult m1 (n1 @ n2))" by (simp add: monom_mult_vars)
-    from p q have pq: "1 \<le> p + q" by auto
-    from Cons(1)[OF m1 n1n2] pq xn1
-    show ?thesis 
-      by (simp only: rec, auto simp: monom_inv_def x)
-  qed
-qed
-
-lemma monom_mult_inj: assumes m: "monom_inv m" and m1: "monom_inv m1" and m2: "monom_inv m2"
-  and eq: "monom_mult m m1 =m monom_mult m m2"
-  shows "m1 =m m2"
-proof -
-  {
-    fix x n 
-    have "sum_var_list (monom_mult m n) x = sum_var_list m x + sum_var_list n x"
-    proof (induct m arbitrary: n, simp add: sum_var_list_def)
-      case (Cons yp m)
-      obtain y p where yp: "yp = (y,p)" by (cases yp, auto)
-      hence id: "sum_var_list (yp # m) x = (if x = y then p else 0) + sum_var_list m x" unfolding sum_var_list_def by auto
-      show ?case
-      proof (cases "List.extract (\<lambda> zq. fst zq = y) n")
-        case None
-        have "sum_var_list (monom_mult (yp # m) n) x = (if x = y then p else 0) + sum_var_list (monom_mult m n) x"
-          by (simp add: yp None sum_var_list_def)
-        thus ?thesis
-          by (simp add: Cons id)
+    case (Cons yq n)
+    then obtain y q where id: "n' = ((y,q) # n)" by (cases yq, auto)
+    from xpm have m: "monom_inv m" and p: "p > 0" and x: "x \<notin> fst ` set m" 
+      and xm: "\<And> z. z \<in> fst ` set m \<Longrightarrow> x \<le> z" 
+      unfolding monom_inv_def by (auto simp: sorted_Cons)
+    from n'[unfolded id] have n: "monom_inv n" and q: "q > 0" and y: "y \<notin> fst ` set n" 
+      and yn: "\<And> z. z \<in> fst ` set n \<Longrightarrow> y \<le> z" 
+      unfolding monom_inv_def by (auto simp: sorted_Cons)
+    show ?thesis
+    proof (cases "x = y")
+      case True
+      hence res: "monom_mult_list ((x, p) # m) n' = (x, p + q) # monom_mult_list m n" 
+        by (simp add: id)
+      from IH(1)[OF id refl True m n] have inv: "monom_inv (monom_mult_list m n)" by simp
+      show ?thesis unfolding res using inv p x y True xm yn
+        by (fastforce simp add: monom_inv_def sorted_Cons monom_list_mult_list_vars)
+    next
+      case False
+      show ?thesis
+      proof (cases "x < y")
+        case True
+        hence res: "monom_mult_list ((x, p) # m) n' = (x,p) # monom_mult_list m n'" 
+          by (auto simp add: id)
+        from IH(2)[OF id refl False True m n'] have inv: "monom_inv (monom_mult_list m n')" .
+        show ?thesis unfolding res using inv p x y True xm yn unfolding id
+          by (fastforce simp add: monom_inv_def sorted_Cons monom_list_mult_list_vars)
       next
-        case (Some res)
-        obtain n1 zq n2 where "res = (n1,zq,n2)" by (cases res, auto)
-        then obtain z q where res: "res = (n1,(z,q),n2)" by (cases zq, auto)
-        from extract_SomeE[OF Some[simplified res]] Some res yp have n: "n = n1 @ (y,q) # n2"
-          and rec: "sum_var_list (monom_mult (yp # m) n) x  = (if x = y then p+q else 0) + sum_var_list (monom_mult m (n1 @ n2)) x" 
-          unfolding sum_var_list_def by auto
-        show ?thesis
-          by (simp only: rec Cons id, simp add: n sum_var_list_def)
+        case gt: False
+        with False have lt: "y < x" by auto        
+        hence res: "monom_mult_list ((x, p) # m) n' = (y,q) # monom_mult_list ((x, p) # m) n" 
+          using False by (auto simp add: id)
+        from lt have zm: "z \<le> x \<Longrightarrow> (z,b) \<notin> set m" for z b using xm[of z] x by force
+        from zm[of y] lt have ym: "(y,b) \<notin> set m" for b by auto
+        from yn have yn': "(a, b) \<in> set n \<Longrightarrow> y \<le> a" for a b by force
+        from IH(3)[OF id refl False gt xpm n] have inv: "monom_inv (monom_mult_list ((x, p) # m) n)" .
+        define xpm where "xpm = ((x,p) # m)" 
+        have xpm': "fst ` set xpm = insert x (fst ` set m)" unfolding xpm_def by auto
+        show ?thesis unfolding res using inv p q x y False gt ym lt xm yn' zm xpm' unfolding id xpm_def[symmetric]
+          by (auto simp add: monom_inv_def sorted_Cons monom_list_mult_list_vars)
       qed
     qed
-  } note main = this
-  from eq main show ?thesis
-    by  (auto simp: eq_monom_sum_var_list[OF m1 m2] eq_monom_sum_var_list[OF monom_mult_inv[OF m m1] monom_mult_inv[OF m m2]])
+  qed
+qed auto
+
+lemma monom_inv_ConsD: "monom_inv (x # xs) \<Longrightarrow> monom_inv xs" 
+  by (auto simp: monom_inv_def sorted_Cons)
+
+lemma sum_var_list_monom_mult_list:  "sum_var_list (monom_mult_list m n) x = sum_var_list m x + sum_var_list n x"
+proof (induct m n rule: monom_mult_list.induct)
+  case (2 x p m n)
+  thus ?case by (cases n; cases "hd n", auto split: if_splits simp: sum_var_list_def)
+qed (auto simp: sum_var_list_def)
+
+lemma monom_mult_list_inj: assumes m: "monom_inv m" and m1: "monom_inv m1" and m2: "monom_inv m2"
+  and eq: "monom_mult_list m m1 = monom_mult_list m m2"
+  shows "m1 = m2"
+proof -
+  from eq sum_var_list_monom_mult_list[of m] show ?thesis
+    by (auto simp: eq_monom_sum_var_list[OF m1 m2] eq_monom_sum_var_list[OF monom_mult_list_inv[OF m m1] monom_mult_list_inv[OF m m2]])
 qed
 
+lemma monom_mult_list[simp]: "eval_monom_list \<alpha> (monom_mult_list m n) = eval_monom_list \<alpha> m * eval_monom_list \<alpha> n"
+  by (induct m n rule: monom_mult_list.induct, auto split: list.splits prod.splits simp: field_simps power_add)
+end
 
-lemma monom_mult[simp]: "eval_monom \<alpha> (monom_mult m n) = eval_monom \<alpha> m * eval_monom \<alpha> n"
-proof (induct m arbitrary: n)
-  case (Cons xp m) note mCons = this
-  show ?case
-  proof (cases xp)
-    case (Pair x p)
-    show ?thesis 
-    proof (cases "List.extract (\<lambda> yq. fst yq = x) n")
-      case None
-      with Cons Pair show ?thesis by (auto simp: field_simps)
-    next
-      case (Some res)
-      obtain n1 yq n2 where "res = (n1,yq,n2)" by (cases res, auto)
-      then obtain y q where res: "res = (n1,(y,q),n2)" by (cases yq, auto)
-      from extract_SomeE[OF Some[simplified res]] Some Pair res have n: "n = n1 @ (x,q) # n2" 
-        and rec: "monom_mult (xp # m) n = (x, p+q) # monom_mult m (n1 @ n2)" by auto
-      show ?thesis by (simp only: rec, simp add: Pair mCons[of "n1 @ n2"] n field_simps power_add)
-    qed
-  qed
-qed simp
+declare monom_mult_list.simps[simp del]
 
-declare monom_mult.simps[simp del]
+typedef (overloaded) 'v monom = "Collect (monom_inv :: 'v :: linorder monom_list \<Rightarrow> bool)"
+  by (rule exI[of _ Nil], auto simp: monom_inv_def)
+
+setup_lifting type_definition_monom
+
+lift_definition eval_monom :: "('v :: linorder,'a :: comm_semiring_1)assign \<Rightarrow> 'v monom \<Rightarrow> 'a"
+  is eval_monom_list .
+
+lift_definition sum_var :: "'v :: linorder monom \<Rightarrow> 'v \<Rightarrow> nat" is sum_var_list .
+
+instantiation monom :: (linorder) comm_monoid_mult
+begin
+
+lift_definition times_monom :: "'a monom \<Rightarrow> 'a monom \<Rightarrow> 'a monom" is monom_mult_list
+  using monom_mult_list_inv by auto
+
+lift_definition one_monom :: "'a monom" is Nil
+  by (auto simp: monom_inv_def)
+
+instance
+proof
+  fix a b c :: "'a monom" 
+  show "a * b * c = a * (b * c)" 
+    by (transfer, auto simp: eq_monom_sum_var_list monom_mult_list_inv sum_var_list_monom_mult_list)
+  show "a * b = b * a"
+    by (transfer, auto simp: eq_monom_sum_var_list monom_mult_list_inv sum_var_list_monom_mult_list)
+  show "1 * a = a" 
+    by (transfer, auto simp: eq_monom_sum_var_list monom_mult_list_inv sum_var_list_monom_mult_list monom_mult_list.simps)
+qed
+end
+
+lemma eq_monom_sum_var: "m = n \<longleftrightarrow> (\<forall> x. sum_var m x = sum_var n x)"
+  by (transfer, auto simp: eq_monom_sum_var_list)
+
+lemma eval_monom_mult[simp]: "eval_monom \<alpha> (m * n) = eval_monom \<alpha> m * eval_monom \<alpha> n"
+  by (transfer, rule monom_mult_list)
+
+lemma sum_var_monom_mult:  "sum_var (m * n) x = sum_var m x + sum_var n x"
+  by (transfer, rule sum_var_list_monom_mult_list)
+
+lemma monom_mult_inj: fixes m1 :: "_ monom"
+  shows "m * m1 = m * m2 \<Longrightarrow> m1 = m2"
+  by (transfer, rule monom_mult_list_inj, auto) 
+
+
+lemma one_monom_inv_sum_var_inv[simp]: "sum_var 1 x = 0" 
+  by (transfer, auto simp: sum_var_list_def)
+
+lemma eval_monom_1[simp]: "eval_monom  \<alpha> 1 = 1" 
+  by (transfer, auto)
+
+lift_definition var_monom :: "'v :: linorder \<Rightarrow> 'v monom" is "\<lambda> x. [(x,1)]" 
+  by (auto simp: monom_inv_def)
+
+lemma var_monom_1[simp]: "var_monom x \<noteq> 1" 
+  by (transfer, auto)
+
+lemma eval_var_monom[simp]: "eval_monom \<alpha> (var_monom x) = \<alpha> x" 
+  by (transfer, auto)
+
+lemma sum_var_monom_var: "sum_var (var_monom x) y = (if x = y then 1 else 0)"
+  by (transfer, auto simp: sum_var_list_def)
 
 text {*
 Polynomials are represented with as sum of monomials multiplied by some coefficient 
@@ -417,36 +397,26 @@ type_synonym ('v,'a)poly = "('v monom \<times> 'a)list"
 text {*
 The polynomials we construct satisfy the following invariants:
 \begin{itemize}
-\item 
-   all monomials satisfy their invariant
 \item all coefficients are non-zero
-\item no two equivalent monomials occur in the list 
+\item the monomial list is distinct 
 \end{itemize}
 *}
 
-fun distinct_eq :: "('a \<Rightarrow> 'a \<Rightarrow> bool) \<Rightarrow> 'a list \<Rightarrow> bool" where
-  "distinct_eq _ [] = True"
-| "distinct_eq eq (x # xs) = ((\<forall> y \<in> set xs. \<not> (eq y x)) \<and> distinct_eq eq xs)"
-
-lemma distinct_eq_append: "distinct_eq eq (xs @ ys) = (distinct_eq eq xs \<and> distinct_eq eq ys \<and> (\<forall> x \<in> set xs. \<forall> y \<in> set ys. \<not> (eq y x)))"
-  by (induct xs, auto)
-
 definition poly_inv :: "('v,'a :: zero)poly \<Rightarrow> bool"
-  where "poly_inv p \<equiv> (\<forall> (m,c) \<in> set p. monom_inv m \<and> c \<noteq> 0) \<and> distinct_eq (\<lambda> (m1,_) (m2,_). m1 =m m2) p"
-
+  where "poly_inv p \<equiv> (\<forall> c \<in> snd ` set p. c \<noteq> 0) \<and> distinct (map fst p)"
 
 abbreviation eval_monomc where "eval_monomc \<alpha> mc \<equiv> eval_monom \<alpha> (fst mc) * (snd mc)"
 
-fun eval_poly :: "('v,'a :: comm_semiring_1)assign \<Rightarrow> ('v,'a)poly \<Rightarrow> 'a"
-where "eval_poly \<alpha> [] = 0"
-   |  "eval_poly \<alpha> (mc # p) = eval_monomc \<alpha> mc + eval_poly \<alpha> p"
+primrec eval_poly :: "('v :: linorder, 'a :: comm_semiring_1)assign \<Rightarrow> ('v,'a)poly \<Rightarrow> 'a" where 
+  "eval_poly \<alpha> [] = 0"
+| "eval_poly \<alpha> (mc # p) = eval_monomc \<alpha> mc + eval_poly \<alpha> p"
 
 
-fun poly_add :: "('v,'a)poly \<Rightarrow> ('v,'a :: semiring_0)poly \<Rightarrow> ('v,'a)poly"
-where "poly_add [] q = q"
-   |  "poly_add ((m,c) # p) q = (case List.extract (\<lambda> mc. fst mc =m m) q of
-                                None \<Rightarrow> (m,c) # poly_add p q
-                              | Some (q1,(_,d),q2) \<Rightarrow> if (c+d = 0) then poly_add p (q1 @ q2) else (m,c+d) # poly_add p (q1 @ q2))"
+fun poly_add :: "('v,'a)poly \<Rightarrow> ('v,'a :: semiring_0)poly \<Rightarrow> ('v,'a)poly" where 
+  "poly_add [] q = q"
+| "poly_add ((m,c) # p) q = (case List.extract (\<lambda> mc. fst mc = m) q of
+    None \<Rightarrow> (m,c) # poly_add p q
+  | Some (q1,(_,d),q2) \<Rightarrow> if (c+d = 0) then poly_add p (q1 @ q2) else (m,c+d) # poly_add p (q1 @ q2))"
 
 lemma eval_poly_append[simp]: "eval_poly \<alpha> (mc1 @ mc2) = eval_poly \<alpha> mc1 + eval_poly \<alpha> mc2"
   by (induct mc1, auto simp: field_simps)
@@ -461,13 +431,13 @@ proof (induct p1 arbitrary: p2)
   obtain m c where mc: "mc = (m,c)" by (cases mc, auto)
   hence m: "m \<in> poly_monoms (mc # p1)" by auto
   show ?case
-  proof (cases "List.extract (\<lambda> nd. fst nd =m m) p2")
+  proof (cases "List.extract (\<lambda> nd. fst nd = m) p2")
     case None
     with Cons m show ?thesis by (auto simp: mc)
   next
     case (Some res)
     obtain q1 md q2 where res: "res = (q1,md,q2)" by (cases res, auto)
-    from extract_SomeE[OF Some[simplified res]] res obtain m' d where q: "p2 = q1 @ (m',d) # q2" and res: "res = (q1,(m',d),q2)" and mm': "m' =m m" by (cases md, auto)
+    from extract_SomeE[OF Some[simplified res]] res obtain d where q: "p2 = q1 @ (m,d) # q2" and res: "res = (q1,(m,d),q2)" by (cases md, auto)
     show ?thesis
       by (simp add: mc Some res, rule subset_trans[OF Cons[of "q1 @ q2"]], auto simp: q)
   qed
@@ -478,82 +448,66 @@ lemma poly_add_inv: "poly_inv p \<Longrightarrow> poly_inv q \<Longrightarrow> p
 proof (induct p arbitrary: q)
   case (Cons mc p)
   obtain m c where mc: "mc = (m,c)" by (cases mc, auto)
-  with Cons(2) have p: "poly_inv p" and m: "monom_inv m" and c: "c \<noteq> 0" and mp: "\<forall> (mm,dd) \<in> set p. (\<not> mm =m m)" unfolding poly_inv_def by auto
+  with Cons(2) have p: "poly_inv p" and c: "c \<noteq> 0" and mp: "\<forall> mm \<in> fst ` set p. (\<not> mm = m)" unfolding poly_inv_def by auto
   show ?case
-  proof (cases "List.extract (\<lambda> mc. fst mc =m m) q")
+  proof (cases "List.extract (\<lambda> mc. fst mc = m) q")
     case None
-    hence mq: "\<forall> (mm,dd) \<in> set q. \<not> mm =m m" by (auto simp: extract_None_iff)
+    hence mq: "\<forall> mm \<in> fst ` set q. \<not> mm = m" by (auto simp: extract_None_iff)
     { 
-      fix mm dd
-      assume "(mm,dd) \<in> set (poly_add p q)"
+      fix mm 
+      assume "mm \<in> fst ` set (poly_add p q)" 
+      then obtain dd where "(mm,dd) \<in> set (poly_add p q)" by auto
       with poly_add_monoms have "mm \<in> poly_monoms p \<or> mm \<in> poly_monoms q" by force
-      hence "\<not> mm =m m"
-      proof
-        assume "mm \<in> poly_monoms p"
-        thus ?thesis using mp  by auto
-      next
-        assume "mm \<in> poly_monoms q"
-        thus ?thesis using mq by auto
-      qed
+      hence "\<not> mm = m" using mp mq by auto
     } note main = this
-    show ?thesis using Cons(1)[OF p Cons(3)] unfolding poly_inv_def by (auto simp add: None mc m c main)
+    show ?thesis using Cons(1)[OF p Cons(3)] unfolding poly_inv_def using main by (auto simp add: None mc c)
   next
     case (Some res)
     obtain q1 md q2 where res: "res = (q1,md,q2)" by (cases res, auto)
-    from extract_SomeE[OF Some[simplified res]] res obtain m' d where q: "q = q1 @ (m',d) # q2" and res: "res = (q1,(m',d),q2)" and mm': "m' =m m" by (cases md, auto)
-    from q Cons(3) have q1q2: "poly_inv (q1 @ q2)" and m': "monom_inv m'" unfolding poly_inv_def by (auto simp: distinct_eq_append)
+    from extract_SomeE[OF Some[simplified res]] res obtain d where q: "q = q1 @ (m,d) # q2" and res: "res = (q1,(m,d),q2)" by (cases md, auto)
+    from q Cons(3) have q1q2: "poly_inv (q1 @ q2)" unfolding poly_inv_def by auto
     from Cons(1)[OF p q1q2]  have main1: "poly_inv (poly_add p (q1 @ q2))" .
     {
-      fix mm dd
-      assume "(mm,dd) \<in> set (poly_add p (q1 @ q2))"
+      fix mm
+      assume "mm \<in> fst ` set (poly_add p (q1 @ q2))"
+      then obtain dd where "(mm,dd) \<in> set (poly_add p (q1 @ q2))" by auto
       with poly_add_monoms have "mm \<in> poly_monoms p \<or> mm \<in> poly_monoms (q1 @ q2)" by force
-      hence "\<not> mm =m m"
+      hence "mm \<noteq> m"
       proof
         assume "mm \<in> poly_monoms p"
         thus ?thesis using mp  by auto
       next
         assume member: "mm \<in> poly_monoms (q1 @ q2)"
-        with q1q2 have mm: "monom_inv mm" unfolding poly_inv_def by auto
         from member have "mm \<in> poly_monoms q1 \<or> mm \<in> poly_monoms q2" by auto
-        hence mmm': "\<not> mm =m m'"
+        thus "mm \<noteq> m"
         proof
           assume "mm \<in> poly_monoms q2"
           with Cons(3)[simplified q]
-          show ?thesis unfolding poly_inv_def by (auto simp: distinct_eq_append)
+          show ?thesis unfolding poly_inv_def by auto
         next
           assume "mm \<in> poly_monoms q1"
           with Cons(3)[simplified q]
-          have "\<not> m' =m mm" unfolding poly_inv_def by (auto simp: distinct_eq_append)
-          thus ?thesis using eq_monom_sym[OF m' mm] by blast
-        qed
-        show ?thesis
-        proof
-          assume "mm =m m"
-          from this mm'[simplified eq_monom_sym[OF m' m]]
-          have "mm =m m'" using eq_monom_trans[OF mm m m'] by blast
-          with mmm' show False by simp
+          show ?thesis unfolding poly_inv_def by auto
         qed
       qed
     } note main2 = this
-    show ?thesis 
-      by (simp add: mc Some res main1, simp add: poly_inv_def m, auto simp: main1[unfolded poly_inv_def] main2)
+    show ?thesis using  main1[unfolded poly_inv_def] main2
+      by (auto simp: poly_inv_def mc Some res)
   qed
 qed simp
-    
-
 
 lemma poly_add[simp]: "eval_poly \<alpha> (poly_add p q) = eval_poly \<alpha> p + eval_poly \<alpha> q"
 proof (induct p arbitrary: q)
   case (Cons mc p)
   obtain m c where mc: "mc = (m,c)" by (cases mc, auto)
   show ?case
-  proof (cases "List.extract (\<lambda> mc. fst mc =m m) q")
+  proof (cases "List.extract (\<lambda> mc. fst mc = m) q")
     case None
     show ?thesis by (simp add: Cons[of q] mc None field_simps)
   next
     case (Some res)
     obtain q1 md q2 where res: "res = (q1,md,q2)" by (cases res, auto)
-    from extract_SomeE[OF Some[simplified res]] res obtain m' d where q: "q = q1 @ (m',d) # q2" and m': "m' =m m" and res: "res = (q1,(m',d),q2)" by (cases md, auto)
+    from extract_SomeE[OF Some[simplified res]] res obtain d where q: "q = q1 @ (m,d) # q2" and res: "res = (q1,(m,d),q2)" by (cases md, auto)
     {
       fix x
       assume c: "c + d = 0"
@@ -562,43 +516,44 @@ proof (induct p arbitrary: q)
       finally have "c * x + d * x = 0" by simp
     } note id = this
     show ?thesis 
-      by (simp add: Cons[of "q1 @ q2"] mc Some res, simp only: q, simp add: eq_monom[OF m'] field_simps, auto simp: field_simps id)
+      by (simp add: Cons[of "q1 @ q2"] mc Some res, simp only: q, simp add: field_simps, auto simp: field_simps id)
   qed
 qed simp
 
 declare poly_add.simps[simp del]
 
-fun monom_mult_poly :: "('v monom \<times> 'a) \<Rightarrow> ('v,'a :: semiring_0)poly \<Rightarrow> ('v,'a)poly"
-where "monom_mult_poly _ [] = []"
-    | "monom_mult_poly (m,c) ((m',d) # p) = (if c * d = 0 then monom_mult_poly (m,c) p else (monom_mult m m', c * d) # monom_mult_poly (m,c) p)"
+fun monom_mult_poly :: "('v :: linorder monom \<times> 'a) \<Rightarrow> ('v,'a :: semiring_0)poly \<Rightarrow> ('v,'a)poly" where 
+  "monom_mult_poly _ [] = []"
+| "monom_mult_poly (m,c) ((m',d) # p) = (if c * d = 0 then monom_mult_poly (m,c) p else (m * m', c * d) # monom_mult_poly (m,c) p)"
 
-lemma monom_mult_poly_inv: assumes m: "monom_inv m" shows "poly_inv p \<Longrightarrow> poly_inv (monom_mult_poly (m,c) p)"
+lemma monom_mult_poly_inv: "poly_inv p \<Longrightarrow> poly_inv (monom_mult_poly (m,c) p)"
 proof (induct p)
   case Nil thus ?case by (simp add: poly_inv_def)
 next
   case (Cons md p)
   obtain m' d where md: "md = (m',d)" by (cases md, auto)
-  with Cons(2) have m': "monom_inv m'" and p: "poly_inv p" unfolding poly_inv_def by auto
+  with Cons(2) have p: "poly_inv p" unfolding poly_inv_def by auto
   from Cons(1)[OF p] have prod: "poly_inv (monom_mult_poly (m,c) p)" .
   {
-    fix mm dd
-    assume one: "(mm,dd) \<in> set (monom_mult_poly (m,c) p)"
-      and two: "mm =m monom_mult m m'"
-    have "poly_monoms (monom_mult_poly (m,c) p) \<subseteq> monom_mult m ` poly_monoms p" 
+    fix mm 
+    assume "mm \<in> fst ` set (monom_mult_poly (m,c) p)" 
+       and two: "mm = m * m'"
+    then obtain dd where one: "(mm,dd) \<in> set (monom_mult_poly (m,c) p)" by auto
+    have "poly_monoms (monom_mult_poly (m,c) p) \<subseteq> op * m ` poly_monoms p" 
     proof (induct p, simp)
       case (Cons md p)
       thus ?case
         by (cases md, auto)
     qed
-    with one have "mm \<in> monom_mult m ` poly_monoms p" by force
-    then obtain mmm where mmm: "mmm \<in> poly_monoms p" and mm: "mm = monom_mult m mmm" by blast
-    from Cons(2)[simplified md] mmm have not1: "\<not> mmm =m m'" and mmm: "monom_inv mmm" unfolding poly_inv_def by (auto simp: distinct_eq_append)
-    from mm two have "monom_mult m mmm =m monom_mult m m'" by simp
-    from monom_mult_inj[OF m mmm m' this] not1 
+    with one have "mm \<in> op * m ` poly_monoms p" by force
+    then obtain mmm where mmm: "mmm \<in> poly_monoms p" and mm: "mm = m * mmm" by blast
+    from Cons(2)[simplified md] mmm have not1: "\<not> mmm = m'" unfolding poly_inv_def by auto
+    from mm two have "m * mmm = m * m'" by simp
+    from monom_mult_inj[OF this] not1 
     have False by simp
   } 
   thus ?case 
-    by (simp add: md prod, intro impI, simp add: poly_inv_def, simp add: monom_mult_inv[OF m m'], auto simp: prod[simplified poly_inv_def])
+    by (simp add: md prod, intro impI, auto simp: poly_inv_def prod[simplified poly_inv_def])
 qed
 
 lemma monom_mult_poly[simp]: "eval_poly \<alpha> (monom_mult_poly mc p) = eval_monomc \<alpha> mc * eval_poly \<alpha> p"
@@ -627,9 +582,9 @@ qed
 
 declare monom_mult_poly.simps[simp del]
 
-fun poly_mult :: "('v,'a :: semiring_0)poly \<Rightarrow> ('v,'a)poly \<Rightarrow> ('v,'a)poly" 
-where "poly_mult [] q = []"
-   |  "poly_mult (mc # p) q = poly_add (monom_mult_poly mc q) (poly_mult p q)"
+fun poly_mult :: "('v :: linorder, 'a :: semiring_0)poly \<Rightarrow> ('v,'a)poly \<Rightarrow> ('v,'a)poly" where 
+  "poly_mult [] q = []"
+| "poly_mult (mc # p) q = poly_add (monom_mult_poly mc q) (poly_mult p q)"
 
 lemma poly_mult_inv: assumes p: "poly_inv p" and q: "poly_inv q"
   shows "poly_inv (poly_mult p q)"
@@ -639,17 +594,13 @@ proof (induct p)
 next
   case (Cons mc p)
   obtain m c where mc: "mc = (m,c)" by (cases mc, auto)
-  with Cons(2) have m: "monom_inv m" and p: "poly_inv p" unfolding poly_inv_def by auto
+  with Cons(2) have p: "poly_inv p" unfolding poly_inv_def by auto
   show ?case
-    by (simp add: mc, rule poly_add_inv[OF monom_mult_poly_inv[OF m q] Cons(1)[OF p]])
+    by (simp add: mc, rule poly_add_inv[OF monom_mult_poly_inv[OF q] Cons(1)[OF p]])
 qed
 
 lemma poly_mult[simp]: "eval_poly \<alpha> (poly_mult p q) = eval_poly \<alpha> p * eval_poly \<alpha> q"
-proof (induct p)
-  case (Cons mc p)
-  thus ?case
-    by (simp add: field_simps)
-qed simp
+  by (induct p, auto simp: field_simps)
 
 declare poly_mult.simps[simp del]
 
@@ -658,8 +609,8 @@ where "zero_poly \<equiv> []"
 
 lemma zero_poly_inv: "poly_inv zero_poly" unfolding zero_poly_def poly_inv_def by auto
 
-definition one_poly :: "('v,'a :: semiring_1)poly"
-where "one_poly \<equiv> [([],1)]"
+definition one_poly :: "('v :: linorder,'a :: semiring_1)poly" where 
+  "one_poly \<equiv> [(1,1)]"
 
 lemma one_poly_inv: "poly_inv one_poly" unfolding one_poly_def poly_inv_def monom_inv_def by auto
 
@@ -668,12 +619,11 @@ lemma poly_zero_add: "poly_add zero_poly p = p" unfolding zero_poly_def using po
 lemma poly_zero_mult: "poly_mult zero_poly p = zero_poly" unfolding zero_poly_def using poly_mult.simps by auto
 
 text {* equality of polynomials *}
-definition eq_poly :: "('v,'a :: comm_semiring_1)poly \<Rightarrow> ('v,'a)poly \<Rightarrow> bool" (infix "=p" 51)
+definition eq_poly :: "('v :: linorder, 'a :: comm_semiring_1)poly \<Rightarrow> ('v,'a)poly \<Rightarrow> bool" (infix "=p" 51)
 where "p =p q \<equiv> \<forall> \<alpha>. eval_poly \<alpha> p = eval_poly \<alpha> q"
 
 lemma poly_one_mult: "poly_mult one_poly p =p p" 
-unfolding eq_poly_def one_poly_def
-by (simp)
+  unfolding eq_poly_def one_poly_def by simp
 
 lemma eq_poly_refl[simp]: "p =p p" unfolding eq_poly_def by auto
 
@@ -693,9 +643,9 @@ lemma poly_distrib: "poly_mult p (poly_add q1 q2) =p poly_add (poly_mult p q1) (
 
 subsection {* Computing normal forms of polynomials *}
 fun
-  poly_of :: "('v,'a :: comm_semiring_1)tpoly \<Rightarrow> ('v,'a)poly"
-where "poly_of (PNum i) = (if i = 0 then [] else [([],i)])"
-    | "poly_of (PVar x) = [([(x,1)],1)]"
+  poly_of :: "('v :: linorder,'a :: comm_semiring_1)tpoly \<Rightarrow> ('v,'a)poly"
+where "poly_of (PNum i) = (if i = 0 then [] else [(1,i)])"
+    | "poly_of (PVar x) = [(var_monom x,1)]"
     | "poly_of (PSum []) = zero_poly" 
     | "poly_of (PSum (p # ps)) = (poly_add (poly_of p) (poly_of (PSum ps)))"
     | "poly_of (PMult []) = one_poly" 
@@ -721,9 +671,9 @@ by (induct p rule: poly_of.induct,
 
 
 subsection {* Powers and substitutions of polynomials *}
-fun poly_power :: "('v,'a :: comm_semiring_1)poly \<Rightarrow> nat \<Rightarrow> ('v,'a)poly"
-where "poly_power _ 0 = one_poly"
-  | "poly_power p (Suc n) = poly_mult p (poly_power p n)"
+fun poly_power :: "('v :: linorder, 'a :: comm_semiring_1)poly \<Rightarrow> nat \<Rightarrow> ('v,'a)poly" where 
+  "poly_power _ 0 = one_poly"
+| "poly_power p (Suc n) = poly_mult p (poly_power p n)"
 
 lemma poly_power[simp]: "eval_poly \<alpha> (poly_power p n) = (eval_poly \<alpha> p) ^ n"
   by (induct n, auto simp: one_poly_def)
@@ -732,15 +682,19 @@ lemma poly_power_inv: assumes p: "poly_inv p"
   shows "poly_inv (poly_power p n)"
   by (induct n, simp add: one_poly_inv, simp add: poly_mult_inv[OF p])
 
-
 declare poly_power.simps[simp del]
 
-fun monom_subst :: "('v \<Rightarrow> ('w,'a :: comm_semiring_1)poly) \<Rightarrow> 'v monom \<Rightarrow> ('w,'a)poly"
-where "monom_subst \<sigma> [] = one_poly"
-  | "monom_subst \<sigma> ((x,p) # m) = poly_mult (poly_power (\<sigma> x) p) (monom_subst \<sigma> m)"
+fun monom_list_subst :: "('v \<Rightarrow> ('w :: linorder,'a :: comm_semiring_1)poly) \<Rightarrow> 'v monom_list \<Rightarrow> ('w,'a)poly" where 
+  "monom_list_subst \<sigma> [] = one_poly"
+| "monom_list_subst \<sigma> ((x,p) # m) = poly_mult (poly_power (\<sigma> x) p) (monom_list_subst \<sigma> m)"
 
-lemma monom_subst_inv: assumes sub: "\<And> x. poly_inv (\<sigma> x)" 
-  shows "poly_inv (monom_subst \<sigma> m)"
+lift_definition monom_list :: "'v :: linorder monom \<Rightarrow> 'v monom_list" is "\<lambda> x. x" .
+
+definition monom_subst :: "('v :: linorder \<Rightarrow> ('w :: linorder,'a :: comm_semiring_1)poly) \<Rightarrow> 'v monom \<Rightarrow> ('w,'a)poly" where 
+  "monom_subst \<sigma> m = monom_list_subst \<sigma> (monom_list m)"  
+
+lemma monom_list_subst_inv: assumes sub: "\<And> x. poly_inv (\<sigma> x)" 
+  shows "poly_inv (monom_list_subst \<sigma> m)"
 proof (induct m)
   case Nil thus ?case by (simp add: one_poly_inv)
 next
@@ -749,14 +703,21 @@ next
   show ?case by (simp add: xp, rule poly_mult_inv[OF poly_power_inv[OF sub] Cons])
 qed
 
+lemma monom_subst_inv: assumes sub: "\<And> x. poly_inv (\<sigma> x)" 
+  shows "poly_inv (monom_subst \<sigma> m)"
+  unfolding monom_subst_def by (rule monom_list_subst_inv[OF sub])
+
 lemma monom_subst[simp]: "eval_poly \<alpha> (monom_subst \<sigma> m) = eval_monom (\<lambda> v. eval_poly \<alpha> (\<sigma> v)) m"
-  by (induct m, simp add: one_poly_def, auto simp: field_simps)
+  unfolding monom_subst_def
+proof (transfer fixing: \<alpha> \<sigma>, clarsimp)
+  fix m 
+  show "monom_inv m \<Longrightarrow> eval_poly \<alpha> (monom_list_subst \<sigma> m) = eval_monom_list (\<lambda>v. eval_poly \<alpha> (\<sigma> v)) m"
+    by (induct m, simp add: one_poly_def, auto simp: field_simps monom_inv_ConsD)
+qed
 
-declare monom_subst.simps[simp del]
-
-fun poly_subst :: "('v \<Rightarrow> ('w,'a :: comm_semiring_1)poly) \<Rightarrow> ('v,'a)poly \<Rightarrow> ('w,'a)poly"
-where "poly_subst \<sigma> [] = zero_poly"
-  | "poly_subst \<sigma> ((m,c) # p) = poly_add (poly_mult [([],c)] (monom_subst \<sigma> m)) (poly_subst \<sigma> p)"
+fun poly_subst :: "('v :: linorder \<Rightarrow> ('w :: linorder,'a :: comm_semiring_1)poly) \<Rightarrow> ('v,'a)poly \<Rightarrow> ('w,'a)poly" where 
+  "poly_subst \<sigma> [] = zero_poly"
+| "poly_subst \<sigma> ((m,c) # p) = poly_add (poly_mult [(1,c)] (monom_subst \<sigma> m)) (poly_subst \<sigma> p)"
 
 lemma poly_subst_inv: assumes sub: "\<And> x. poly_inv (\<sigma> x)" and p: "poly_inv p"
   shows "poly_inv (poly_subst \<sigma> p)"
@@ -767,7 +728,7 @@ next
   case (Cons mc p)
   obtain m c where mc: "mc = (m,c)" by (cases mc, auto)
   with Cons(2) have c: "c \<noteq> 0" and p: "poly_inv p" unfolding poly_inv_def by auto
-  from c have c: "poly_inv [([],c)]" unfolding poly_inv_def monom_inv_def by auto
+  from c have c: "poly_inv [(1,c)]" unfolding poly_inv_def monom_inv_def by auto
   show ?case 
     by (simp add: mc, rule poly_add_inv[OF poly_mult_inv[OF c monom_subst_inv[OF sub]] Cons(1)[OF p]])
 qed
@@ -776,30 +737,76 @@ lemma poly_subst: "eval_poly \<alpha> (poly_subst \<sigma> p) = eval_poly (\<lam
   by (induct p, simp add: zero_poly_def, auto simp: field_simps)
 
 lemma eval_poly_subst: 
-      assumes eq: "\<And> w. f w = eval_poly g (q w)"
-      shows "eval_poly f p = eval_poly g (poly_subst q p)" 
+  assumes eq: "\<And> w. f w = eval_poly g (q w)"
+  shows "eval_poly f p = eval_poly g (poly_subst q p)" 
 proof (induct p)
   case Nil thus ?case by (simp add: zero_poly_def)
 next
   case (Cons mc p)
   obtain m c where mc: "mc = (m,c)" by (cases mc, auto)
   have id: "eval_monom f m =  eval_monom (\<lambda>v. eval_poly g (q v)) m"
-  proof (induct m)
-    case (Cons wp m)
-    obtain w p where wp: "wp = (w,p)" by (cases wp, auto)
-    show ?case
-      by (simp add: wp Cons eq)
-  qed simp
+  proof (transfer fixing: f g q, clarsimp)
+    fix m
+    show "eval_monom_list f m = eval_monom_list (\<lambda>v. eval_poly g (q v)) m"
+    proof (induct m)
+      case (Cons wp m)
+      obtain w p where wp: "wp = (w,p)" by (cases wp, auto)
+      show ?case
+        by (simp add: wp Cons eq)
+    qed simp
+  qed
   show ?case
     by (simp add: mc Cons id, simp add: field_simps)
 qed
 
-(* the list of variables occurring in p *)
-definition poly_vars_list :: "('v,'a)poly \<Rightarrow> 'v list"
-where "poly_vars_list p = remdups (concat (map (map fst o fst) p))"
+lift_definition monom_vars_list :: "'v :: linorder monom \<Rightarrow> 'v list" is "map fst" .
 
-definition poly_vars :: "('v,'a)poly \<Rightarrow> 'v set"
-where "poly_vars p = set (concat (map (map fst o fst) p))"
+lemma monom_vars_list_subst: assumes "\<And> w. w \<in> set (monom_vars_list m) \<Longrightarrow> f w = g w" 
+  shows "monom_subst f m = monom_subst g m" 
+  unfolding monom_subst_def using assms
+proof (transfer fixing: f g)
+  fix m :: "'a monom_list" 
+  assume eq: "\<And>w. w \<in> set (map fst m) \<Longrightarrow> f w = g w" 
+  thus "monom_list_subst f m = monom_list_subst g m" 
+  proof (induct m)
+    case (Cons wn m)
+    hence rec: "monom_list_subst f m = monom_list_subst g m" and eq: "f (fst wn) = g (fst wn)" by auto
+    show ?case
+    proof (cases wn)
+      case (Pair w n)
+      with eq rec show ?thesis by auto
+    qed
+  qed simp
+qed
+
+lemma eval_monom_vars_list: assumes "\<And> x. x \<in> set (monom_vars_list xs) \<Longrightarrow> \<alpha> x = \<beta> x"
+  shows "eval_monom \<alpha> xs = eval_monom \<beta> xs" using assms
+proof (transfer fixing: \<alpha> \<beta>)
+  fix xs :: "'a monom_list" 
+  assume eq: "\<And>w. w \<in> set (map fst xs) \<Longrightarrow> \<alpha> w = \<beta> w" 
+  thus "eval_monom_list \<alpha> xs = eval_monom_list \<beta> xs" 
+  proof (induct xs)
+    case (Cons xi xs)
+    hence IH: "eval_monom_list \<alpha> xs = eval_monom_list \<beta> xs" by auto
+    obtain x i where xi: "xi = (x,i)" by force
+    from Cons(2) xi have "\<alpha> x = \<beta> x" by auto
+    with IH show ?case unfolding xi by auto
+  qed simp
+qed
+
+definition monom_vars where "monom_vars m = set (monom_vars_list m)" 
+
+lemma monom_vars_eval_monom: 
+  "(\<And> x. x \<in> monom_vars m \<Longrightarrow> f x = g x) \<Longrightarrow> eval_monom f m = eval_monom g m"
+  by (rule eval_monom_vars_list, auto simp: monom_vars_def)
+
+
+(* the list of variables occurring in p *)
+definition poly_vars_list :: "('v :: linorder,'a)poly \<Rightarrow> 'v list" where 
+  "poly_vars_list p = remdups (concat (map (monom_vars_list o fst) p))"
+
+definition poly_vars :: "('v :: linorder,'a)poly \<Rightarrow> 'v set" where 
+  "poly_vars p = set (concat (map (monom_vars_list o fst) p))"
 
 lemma poly_vars_list[simp]: "set (poly_vars_list p) = poly_vars p" 
   unfolding poly_vars_list_def poly_vars_def by auto
@@ -813,19 +820,9 @@ proof (induct p)
   show ?case
   proof (cases mc)
     case (Pair m c)
-    with Cons(2) have "\<And> w. w \<in> set (map fst m) \<Longrightarrow> f w = g w" unfolding poly_vars_def by auto
+    with Cons(2) have "\<And> w. w \<in> set (monom_vars_list m) \<Longrightarrow> f w = g w" unfolding poly_vars_def by auto
     hence "monom_subst f m = monom_subst g m"
-    proof (induct m)
-      case Nil thus ?case by (simp add: monom_subst.simps)
-    next
-      case (Cons wn m)
-      hence rec: "monom_subst f m = monom_subst g m" and eq: "f (fst wn) = g (fst wn)" by auto
-      show ?case
-      proof (cases wn)
-        case (Pair w n)
-        with eq rec show ?thesis by (auto simp: monom_subst.simps)
-      qed
-    qed
+      by (rule monom_vars_list_subst)
     with rec Pair show ?thesis by auto
   qed
 qed simp
@@ -838,6 +835,7 @@ proof (rule poly_vars)
   thus "f w = g w" using pv diff by (cases "v = w", auto)
 qed
 
+
 lemma eval_poly_vars: assumes "\<And> x. x \<in> poly_vars p \<Longrightarrow> \<alpha> x = \<beta> x"
   shows "eval_poly \<alpha> p = eval_poly \<beta> p"
 using assms
@@ -848,17 +846,9 @@ next
   from Cons(2) have "\<And> x. x \<in> poly_vars p \<Longrightarrow> \<alpha> x = \<beta> x" unfolding poly_vars_def by auto
   from Cons(1)[OF this] have IH: "eval_poly \<alpha> p = eval_poly \<beta> p" .
   obtain xs c where m: "m = (xs,c)" by force
-  from Cons(2) have "\<And> x. x \<in> set (map fst xs) \<Longrightarrow> \<alpha> x = \<beta> x" unfolding poly_vars_def m by auto
+  from Cons(2) have "\<And> x. x \<in> set (monom_vars_list xs) \<Longrightarrow> \<alpha> x = \<beta> x" unfolding poly_vars_def m by auto
   hence "eval_monom \<alpha> xs = eval_monom \<beta> xs"
-  proof (induct xs)
-    case Nil thus ?case by simp
-  next
-    case (Cons xi xs)
-    hence IH: "eval_monom \<alpha> xs = eval_monom \<beta> xs" by auto
-    obtain x i where xi: "xi = (x,i)" by force
-    from Cons(2) xi have "\<alpha> x = \<beta> x" by auto
-    with IH show ?case unfolding xi by auto
-  qed
+    by (rule eval_monom_vars_list)
   thus ?case unfolding eval_poly.simps IH m by auto
 qed
 
@@ -874,7 +864,7 @@ subsection {*
 definition pos_assign :: "('v,'a :: ordered_semiring_0)assign \<Rightarrow> bool"
 where "pos_assign \<alpha> = (\<forall> x. \<alpha> x \<ge> 0)"
 
-definition poly_ge :: "('v,'a :: poly_carrier)poly \<Rightarrow> ('v,'a)poly \<Rightarrow> bool" (infix "\<ge>p" 51)
+definition poly_ge :: "('v :: linorder,'a :: poly_carrier)poly \<Rightarrow> ('v,'a)poly \<Rightarrow> bool" (infix "\<ge>p" 51)
 where "p \<ge>p q = (\<forall> \<alpha>. pos_assign \<alpha> \<longrightarrow> eval_poly \<alpha> p \<ge> eval_poly \<alpha> q)"
 
 lemma poly_ge_refl[simp]: "p \<ge>p p"
@@ -884,9 +874,9 @@ lemma poly_ge_trans[trans]: "\<lbrakk>p1 \<ge>p p2; p2 \<ge>p p3\<rbrakk> \<Long
 unfolding poly_ge_def using ge_trans by blast
 
 
-lemma pos_assign_monom: fixes \<alpha> :: "('v,'a :: poly_carrier)assign"
+lemma pos_assign_monom_list: fixes \<alpha> :: "('v :: linorder, 'a :: poly_carrier)assign"
   assumes pos: "pos_assign \<alpha>"
-  shows "eval_monom \<alpha> m \<ge> 0"
+  shows "eval_monom_list \<alpha> m \<ge> 0"
 proof (induct m)
   case Nil thus ?case by (simp add: one_ge_zero)
 next
@@ -909,6 +899,12 @@ next
   qed
 qed
 
+lemma pos_assign_monom: fixes \<alpha> :: "('v :: linorder, 'a :: poly_carrier)assign"
+  assumes pos: "pos_assign \<alpha>"
+  shows "eval_monom \<alpha> m \<ge> 0"
+  by (transfer fixing: \<alpha>, rule pos_assign_monom_list[OF pos])
+
+
 lemma pos_assign_poly:   assumes pos: "pos_assign \<alpha>"
   and p: "p \<ge>p zero_poly"
   shows "eval_poly \<alpha> p \<ge> 0"
@@ -928,12 +924,12 @@ using assms unfolding poly_ge_def zero_poly_def by (auto simp: times_left_mono)
 context poly_order_carrier
 begin
 
-definition poly_gt :: "('v,'a)poly \<Rightarrow> ('v,'a)poly \<Rightarrow> bool" (infix ">p" 51)
+definition poly_gt :: "('v :: linorder,'a)poly \<Rightarrow> ('v,'a)poly \<Rightarrow> bool" (infix ">p" 51)
 where "p >p q = (\<forall> \<alpha>. pos_assign \<alpha> \<longrightarrow> eval_poly \<alpha> p \<succ> eval_poly \<alpha> q)"
 
 lemma poly_gt_imp_poly_ge: "p >p q \<Longrightarrow> p \<ge>p q" unfolding poly_ge_def poly_gt_def using gt_imp_ge by blast
 
-abbreviation poly_GT :: "('v,'a)poly rel"
+abbreviation poly_GT :: "('v :: linorder,'a)poly rel"
 where "poly_GT \<equiv> {(p,q) | p q. p >p q \<and> q \<ge>p zero_poly}"
 
 lemma poly_compat: "\<lbrakk>p1 \<ge>p p2; p2 >p p3\<rbrakk> \<Longrightarrow> p1 >p p3"
@@ -947,7 +943,7 @@ unfolding poly_gt_def using gt_trans by blast
 
 lemma poly_GT_SN: "SN poly_GT"
 proof
-  fix f :: "nat \<Rightarrow> ('c,'a)poly"
+  fix f :: "nat \<Rightarrow> ('c :: linorder,'a)poly"
   assume f: "\<forall> i. (f i, f (Suc i)) \<in> poly_GT"
   have pos: "pos_assign ((\<lambda> x. 0) :: ('v,'a)assign)" (is "pos_assign ?ass") unfolding pos_assign_def using ge_refl by auto
   obtain g where g: "\<And> i. g i = eval_poly ?ass (f i)" by auto
@@ -958,29 +954,31 @@ end
 
 text {* monotonicity of polynomials *}
 
-lemma eval_monom_mono: assumes fg: "\<And> x. (f :: ('v,'a :: poly_carrier)assign) x \<ge> g x" 
+lemma eval_monom_list_mono: assumes fg: "\<And> x. (f :: ('v :: linorder,'a :: poly_carrier)assign) x \<ge> g x" 
   and g: "\<And> x. g x \<ge> 0"
-  shows "eval_monom f m \<ge> eval_monom g m" "eval_monom g m \<ge> 0"
-proof - 
-  have "eval_monom f m \<ge> eval_monom g m \<and> eval_monom g m \<ge> 0"
-  proof (induct m)
-    case Nil show ?case using one_ge_zero by (auto simp: ge_refl)
-  next
-    case (Cons xd m)
-    hence IH1: " eval_monom f m \<ge> eval_monom g m" and IH2: "eval_monom g m \<ge> 0" by auto
-    obtain x d where xd: "xd = (x,d)" by force
-    from pow_mono[OF fg g, of x d] have fgd: "f x ^ d \<ge> g x ^ d" and gd: "g x ^ d \<ge> 0" by auto
-    show ?case unfolding xd eval_monom.simps
-    proof (rule conjI, rule ge_trans[OF times_left_mono[OF pow_ge_zero IH1] times_right_mono[OF IH2 fgd]])
-      show "f x \<ge> 0" by (rule ge_trans[OF fg g])
-      show "eval_monom g m * g x ^ d \<ge> 0"
-        by (rule mult_ge_zero[OF IH2 gd])
-    qed
+  shows "eval_monom_list f m \<ge> eval_monom_list g m" "eval_monom_list g m \<ge> 0"
+proof (atomize(full), induct m)
+  case Nil show ?case using one_ge_zero by (auto simp: ge_refl)
+next
+  case (Cons xd m)
+  hence IH1: " eval_monom_list f m \<ge> eval_monom_list g m" and IH2: "eval_monom_list g m \<ge> 0" by auto
+  obtain x d where xd: "xd = (x,d)" by force
+  from pow_mono[OF fg g, of x d] have fgd: "f x ^ d \<ge> g x ^ d" and gd: "g x ^ d \<ge> 0" by auto
+  show ?case unfolding xd eval_monom_list.simps
+  proof (rule conjI, rule ge_trans[OF times_left_mono[OF pow_ge_zero IH1] times_right_mono[OF IH2 fgd]])
+    show "f x \<ge> 0" by (rule ge_trans[OF fg g])
+    show "eval_monom_list g m * g x ^ d \<ge> 0"
+      by (rule mult_ge_zero[OF IH2 gd])
   qed
-  thus "eval_monom f m \<ge> eval_monom g m" "eval_monom g m \<ge> 0" by auto
 qed
 
-definition poly_weak_mono_all :: "('v,'a :: poly_carrier)poly \<Rightarrow> bool" where 
+lemma eval_monom_mono: assumes fg: "\<And> x. (f :: ('v :: linorder,'a :: poly_carrier)assign) x \<ge> g x" 
+  and g: "\<And> x. g x \<ge> 0"
+shows "eval_monom f m \<ge> eval_monom g m" "eval_monom g m \<ge> 0"
+  by (atomize(full), transfer fixing: f g, insert eval_monom_list_mono[of g f, OF fg g], auto)
+
+
+definition poly_weak_mono_all :: "('v :: linorder,'a :: poly_carrier)poly \<Rightarrow> bool" where 
   "poly_weak_mono_all p \<equiv> \<forall> (\<alpha> :: ('v,'a)assign) \<beta>. (\<forall> x. \<alpha> x \<ge> \<beta> x) 
     \<longrightarrow> pos_assign \<beta> \<longrightarrow> eval_poly \<alpha> p \<ge> eval_poly \<beta> p"
 
@@ -1003,7 +1001,7 @@ next
   qed
 qed
 
-definition poly_weak_mono :: "('v,'a :: poly_carrier)poly \<Rightarrow> 'v \<Rightarrow> bool" where 
+definition poly_weak_mono :: "('v :: linorder,'a :: poly_carrier)poly \<Rightarrow> 'v \<Rightarrow> bool" where 
   "poly_weak_mono p v \<equiv> \<forall> (\<alpha> :: ('v,'a)assign) \<beta>. (\<forall> x. v \<noteq> x \<longrightarrow> \<alpha> x = \<beta> x) \<longrightarrow> pos_assign \<beta> \<longrightarrow> \<alpha> v \<ge> \<beta> v \<longrightarrow> eval_poly \<alpha> p \<ge> eval_poly \<beta> p"
 
 lemma poly_weak_mono_E: assumes p: "poly_weak_mono p v"
@@ -1031,7 +1029,7 @@ next
   show "pos_assign \<alpha> \<Longrightarrow> eval_poly \<alpha> (f x) = eval_poly \<alpha> (g x)" using fgw[OF v] unfolding poly_ge_def by auto
 qed
 
-definition poly_weak_anti_mono :: "('v,'a :: poly_carrier)poly \<Rightarrow> 'v \<Rightarrow> bool" where 
+definition poly_weak_anti_mono :: "('v :: linorder,'a :: poly_carrier)poly \<Rightarrow> 'v \<Rightarrow> bool" where 
   "poly_weak_anti_mono p v \<equiv> \<forall> (\<alpha> :: ('v,'a)assign) \<beta>. (\<forall> x. v \<noteq> x \<longrightarrow> \<alpha> x = \<beta> x) \<longrightarrow> pos_assign \<beta> \<longrightarrow> \<alpha> v \<ge> \<beta> v \<longrightarrow> eval_poly \<beta> p \<ge> eval_poly \<alpha> p"
 
 lemma poly_weak_anti_mono_E: assumes p: "poly_weak_anti_mono p v"
@@ -1059,7 +1057,7 @@ next
   show "pos_assign \<alpha> \<Longrightarrow> eval_poly \<alpha> (f x) = eval_poly \<alpha> (g x)" using fgw[OF v] unfolding poly_ge_def by auto
 qed
 
-lemma poly_weak_mono: fixes p :: "('v,'a :: poly_carrier)poly"
+lemma poly_weak_mono: fixes p :: "('v :: linorder,'a :: poly_carrier)poly"
   assumes mono: "\<And> v. v \<in> poly_vars p \<Longrightarrow> poly_weak_mono p v"
   shows "poly_weak_mono_all p"
 unfolding poly_weak_mono_all_def
@@ -1102,7 +1100,7 @@ proof (intro allI impI)
   show "eval_poly \<alpha> p \<ge> eval_poly \<beta> p" .
 qed  
 
-lemma poly_weak_mono_all: fixes p :: "('v,'a :: poly_carrier)poly" 
+lemma poly_weak_mono_all: fixes p :: "('v :: linorder,'a :: poly_carrier)poly" 
   assumes p: "poly_weak_mono_all p"
   shows "poly_weak_mono p v"
 unfolding poly_weak_mono_def
@@ -1120,7 +1118,7 @@ proof (intro allI impI)
 qed
 
 lemma poly_weak_mono_all_pos: 
-  fixes p :: "('v,'a :: poly_carrier)poly"
+  fixes p :: "('v :: linorder,'a :: poly_carrier)poly"
   assumes pos_at_zero: "eval_poly (\<lambda> w. 0) p \<ge> 0"
   and mono: "poly_weak_mono_all p"
   shows "p \<ge>p zero_poly"
@@ -1146,7 +1144,7 @@ qed
 context poly_order_carrier
 begin
 
-definition poly_strict_mono :: "('v,'a)poly \<Rightarrow> 'v \<Rightarrow> bool" where 
+definition poly_strict_mono :: "('v :: linorder,'a)poly \<Rightarrow> 'v \<Rightarrow> bool" where 
   "poly_strict_mono p v \<equiv> \<forall> (\<alpha> :: ('v,'a)assign) \<beta>. (\<forall> x. (v \<noteq> x \<longrightarrow> \<alpha> x = \<beta> x)) \<longrightarrow> pos_assign \<beta> \<longrightarrow> \<alpha> v \<succ> \<beta> v \<longrightarrow> eval_poly \<alpha> p \<succ> eval_poly \<beta> p"
 
 lemma poly_strict_mono_E: assumes p: "poly_strict_mono p v"
@@ -1178,7 +1176,7 @@ lemma poly_add_gt_mono: assumes "p1 >p p2" shows "poly_add p1 q >p poly_add p2 q
 using assms unfolding poly_gt_def by (auto simp: field_simps plus_gt_left_mono)
 
 lemma poly_mult_gt_mono: 
-  fixes q :: "('v,'a)poly"
+  fixes q :: "('v :: linorder,'a)poly"
   assumes gt: "p1 >p p2" and mono: "q \<ge>p one_poly"
   shows "poly_mult p1 q >p poly_mult p2 q"
 proof (unfold poly_gt_def, intro impI allI)
@@ -1193,23 +1191,34 @@ end
 
 subsection {* Degree of polynomials *}
 
-definition monom_degree :: "'v monom \<Rightarrow> nat" where 
-  "monom_degree xps \<equiv> sum_list (map snd xps)"
+definition monom_list_degree :: "'v monom_list \<Rightarrow> nat" where 
+  "monom_list_degree xps \<equiv> sum_list (map snd xps)"
 
-definition poly_degree :: "('v,'a) poly \<Rightarrow> nat" where
+lift_definition monom_degree :: "'v :: linorder monom \<Rightarrow> nat" is monom_list_degree .
+
+definition poly_degree :: "(_,'a) poly \<Rightarrow> nat" where
   "poly_degree p \<equiv> max_list (map (\<lambda> (m,c). monom_degree m) p)"
 
 definition poly_coeff_sum :: "('v,'a :: ordered_ab_semigroup) poly \<Rightarrow> 'a" where
   "poly_coeff_sum p \<equiv> sum_list (map (\<lambda> mc. max 0 (snd mc)) p)"
 
-lemma monom_degree: "eval_monom (\<lambda> _. x) m = x ^ monom_degree m"
-  unfolding monom_degree_def
+lemma monom_list_degree: "eval_monom_list (\<lambda> _. x) m = x ^ monom_list_degree m"
+  unfolding monom_list_degree_def
 proof (induct m)
   case Nil show ?case by simp
 next 
   case (Cons mc m)
   thus ?case by (cases mc, auto simp: power_add field_simps)
 qed
+
+lemma monom_list_var_monom[simp]: "monom_list (var_monom x) = [(x,1)]" 
+  by (transfer, simp)
+
+lemma monom_list_1[simp]: "monom_list 1 = []" 
+  by (transfer, simp)
+
+lemma monom_degree: "eval_monom (\<lambda> _. x) m = x ^ monom_degree m"
+  by (transfer, rule monom_list_degree)
 
 lemma poly_coeff_sum: "poly_coeff_sum p \<ge> 0"
   unfolding poly_coeff_sum_def
@@ -1258,20 +1267,20 @@ subsection {* Executable and sufficient criteria to compare polynomials and ensu
 
 text {* poly\_split extracts the coefficient for a given monomial and returns additionally the remaining polynomial *}
 definition poly_split :: "('v monom) \<Rightarrow> ('v,'a :: zero)poly \<Rightarrow> 'a \<times> ('v,'a)poly" 
-  where "poly_split m p \<equiv> case List.extract (\<lambda> (n,_). m =m n) p of None \<Rightarrow> (0,p) | Some (p1,(_,c),p2) \<Rightarrow> (c, p1 @ p2)"
+  where "poly_split m p \<equiv> case List.extract (\<lambda> (n,_). m = n) p of None \<Rightarrow> (0,p) | Some (p1,(_,c),p2) \<Rightarrow> (c, p1 @ p2)"
 
 lemma poly_split: assumes "poly_split m p = (c,q)"
   shows "p =p (m,c) # q"
-proof (cases "List.extract (\<lambda> (n,_). m =m n) p")
+proof (cases "List.extract (\<lambda> (n,_). m = n) p")
   case None
   with assms have "(c,q) = (0,p)" unfolding poly_split_def by auto
   thus ?thesis unfolding eq_poly_def by auto
 next
   case (Some res)
   obtain p1 mc p2 where "res = (p1,mc,p2)" by (cases res, auto)
-  with extract_SomeE[OF Some[simplified this]] obtain a m' where p: "p = p1 @ (m',a) # p2" and m': "m =m m'" and res: "res = (p1,(m',a),p2)" by (cases mc, auto)
+  with extract_SomeE[OF Some[simplified this]] obtain a where p: "p = p1 @ (m,a) # p2" and res: "res = (p1,(m,a),p2)" by (cases mc, auto)
   from Some res assms have c: "c = a" and q: "q = p1 @ p2" unfolding poly_split_def by auto
-  show ?thesis unfolding eq_poly_def by (simp add: p c q eq_monom[OF m'] field_simps)
+  show ?thesis unfolding eq_poly_def by (simp add: p c q field_simps)
 qed 
 
 lemma poly_split_eval: assumes "poly_split m p = (c,q)" 
@@ -1279,13 +1288,13 @@ lemma poly_split_eval: assumes "poly_split m p = (c,q)"
 using poly_split[OF assms] unfolding eq_poly_def by auto
 
 (* we assume that the polynomial invariant is present, otherwise this check might fail, e.g., on 0 =p 0 + 0 *)
-fun check_poly_eq :: "('v,'a :: semiring_0)poly \<Rightarrow> ('v,'a)poly \<Rightarrow> bool"
-where "check_poly_eq [] q = (q = [])"
-    | "check_poly_eq ((m,c) # p) q = (case List.extract (\<lambda> nd. fst nd =m m) q of
-                                         None \<Rightarrow> False
-                                       | Some (q1,(_,d),q2) \<Rightarrow> c = d \<and> check_poly_eq p (q1 @ q2))"
+fun check_poly_eq :: "('v,'a :: semiring_0)poly \<Rightarrow> ('v,'a)poly \<Rightarrow> bool" where 
+  "check_poly_eq [] q = (q = [])"
+| "check_poly_eq ((m,c) # p) q = (case List.extract (\<lambda> nd. fst nd = m) q of
+       None \<Rightarrow> False
+     | Some (q1,(_,d),q2) \<Rightarrow> c = d \<and> check_poly_eq p (q1 @ q2))"
 
-lemma check_poly_eq: fixes p :: "('v,'a :: poly_carrier)poly"
+lemma check_poly_eq: fixes p :: "('v :: linorder,'a :: poly_carrier)poly"
   assumes chk: "check_poly_eq p q"
   shows "p =p q" unfolding eq_poly_def
 proof
@@ -1298,17 +1307,17 @@ proof
     case (Cons mc p)
     obtain m c where mc: "mc = (m,c)" by (cases mc, auto)
     show ?case
-    proof (cases "List.extract (\<lambda> mc. fst mc =m m) q")
+    proof (cases "List.extract (\<lambda> mc. fst mc = m) q")
       case None
       with Cons(2) show ?thesis unfolding mc by simp
     next
       case (Some res)
       obtain q1 md q2 where "res = (q1,md,q2)" by (cases res, auto)
-      with extract_SomeE[OF Some[simplified this]] obtain m' d where q: "q = q1 @ (m',d) # q2" and m': "m' =m m" and res: "res = (q1,(m',d),q2)" 
+      with extract_SomeE[OF Some[simplified this]] obtain d where q: "q = q1 @ (m,d) # q2" and res: "res = (q1,(m,d),q2)" 
         by (cases md, auto)
       from Cons(2) Some mc res have rec: "check_poly_eq p (q1 @ q2)" and c: "c = d" by auto
       from Cons(1)[OF rec] have p: "eval_poly \<alpha> p = eval_poly \<alpha> (q1 @ q2)" .
-      show ?thesis unfolding mc eval_poly.simps c p q using eq_monom[OF m', of \<alpha>] by (simp add: ac_simps)
+      show ?thesis unfolding mc eval_poly.simps c p q by (simp add: ac_simps)
     qed
   qed
 qed
@@ -1316,13 +1325,13 @@ qed
 declare check_poly_eq.simps[simp del]
 
 
-fun check_poly_ge :: "('v,'a :: ordered_semiring_0)poly \<Rightarrow> ('v,'a)poly \<Rightarrow> bool"
-where "check_poly_ge [] q = list_all (\<lambda> (_,d). 0 \<ge> d) q"
-    | "check_poly_ge ((m,c) # p) q = (case List.extract (\<lambda> nd. fst nd =m m) q of
-                                         None \<Rightarrow> c \<ge> 0 \<and> check_poly_ge p q
-                                       | Some (q1,(_,d),q2) \<Rightarrow> c \<ge> d \<and> check_poly_ge p (q1 @ q2))"
+fun check_poly_ge :: "('v,'a :: ordered_semiring_0)poly \<Rightarrow> ('v,'a)poly \<Rightarrow> bool" where 
+  "check_poly_ge [] q = list_all (\<lambda> (_,d). 0 \<ge> d) q"
+| "check_poly_ge ((m,c) # p) q = (case List.extract (\<lambda> nd. fst nd = m) q of
+     None \<Rightarrow> c \<ge> 0 \<and> check_poly_ge p q
+   | Some (q1,(_,d),q2) \<Rightarrow> c \<ge> d \<and> check_poly_ge p (q1 @ q2))"
 
-lemma check_poly_ge: fixes p :: "('v,'a :: poly_carrier)poly"
+lemma check_poly_ge: fixes p :: "('v :: linorder,'a :: poly_carrier)poly"
   shows "check_poly_ge p q \<Longrightarrow> p \<ge>p q"
 proof (induct p arbitrary: q)
   case Nil
@@ -1354,7 +1363,7 @@ next
   case (Cons mc p)
   obtain m c where mc: "mc = (m,c)" by (cases mc, auto)
   show ?case
-  proof (cases "List.extract (\<lambda> mc. fst mc =m m) q")
+  proof (cases "List.extract (\<lambda> mc. fst mc = m) q")
     case None
     with Cons(2) have rec: "check_poly_ge p q" and c: "c \<ge> 0" using mc by auto
     from Cons(1)[OF rec] have rec: "p \<ge>p q" .
@@ -1371,7 +1380,7 @@ next
   next
     case (Some res)
     obtain q1 md q2 where "res = (q1,md,q2)" by (cases res, auto)
-    with extract_SomeE[OF Some[simplified this]] obtain m' d where q: "q = q1 @ (m',d) # q2" and m': "m' =m m" and res: "res = (q1,(m',d),q2)" 
+    with extract_SomeE[OF Some[simplified this]] obtain d where q: "q = q1 @ (m,d) # q2" and res: "res = (q1,(m,d),q2)" 
       by (cases md, auto)
     from Cons(2) Some mc res have rec: "check_poly_ge p (q1 @ q2)" and c: "c \<ge> d" by auto
     from Cons(1)[OF rec] have p: "p \<ge>p q1 @ q2" .
@@ -1379,9 +1388,9 @@ next
     proof (simp only: mc, unfold poly_ge_def, intro allI impI)
       fix \<alpha> :: "('v,'a)assign"
       assume pos: "pos_assign \<alpha>"
-      have ge: "eval_monom \<alpha> m * c \<ge> eval_monom \<alpha> m' * d"
+      have ge: "eval_monom \<alpha> m * c \<ge> eval_monom \<alpha> m * d"
         using times_right_mono[OF pos_assign_monom[OF pos, of m] c] 
-          eq_monom[OF m', of \<alpha>] by simp
+          by simp
       from p have ge2: "eval_poly \<alpha> p \<ge> eval_poly \<alpha> (q1 @ q2)" unfolding poly_ge_def using pos by auto
       show "eval_poly \<alpha> ((m,c) # p) \<ge> eval_poly \<alpha> q" using ge_trans[OF plus_left_mono[OF ge] plus_right_mono[OF ge2]]
         by (simp add: q field_simps)
@@ -1394,7 +1403,7 @@ declare check_poly_ge.simps[simp del]
 definition check_poly_weak_mono_all :: "('v,'a :: ordered_semiring_0)poly \<Rightarrow> bool"
 where "check_poly_weak_mono_all p \<equiv> list_all (\<lambda> (m,c). c \<ge> 0) p"
 
-lemma check_poly_weak_mono_all: fixes p :: "('v,'a :: poly_carrier)poly"
+lemma check_poly_weak_mono_all: fixes p :: "('v :: linorder,'a :: poly_carrier)poly"
   assumes "check_poly_weak_mono_all p" shows  "poly_weak_mono_all p"
 unfolding poly_weak_mono_all_def
 proof (intro allI impI)
@@ -1435,22 +1444,22 @@ qed
 
 text {* better check for weak monotonicity for discrete carriers: 
    $p$ is monotone in $v$ if $p(\ldots v+1 \ldots) \geq p(\ldots v \ldots)$ *}
-definition check_poly_weak_mono_discrete :: "('v,'a :: poly_carrier)poly \<Rightarrow> 'v \<Rightarrow> bool"
+definition check_poly_weak_mono_discrete :: "('v :: linorder,'a :: poly_carrier)poly \<Rightarrow> 'v \<Rightarrow> bool"
   where "check_poly_weak_mono_discrete p v \<equiv> check_poly_ge (poly_subst (\<lambda> w. poly_of (if w = v then PSum [PNum 1, PVar v] else PVar w)) p) p"
 
-definition check_poly_weak_mono_and_pos :: "bool \<Rightarrow> ('v,'a :: poly_carrier)poly \<Rightarrow> bool"
+definition check_poly_weak_mono_and_pos :: "bool \<Rightarrow> ('v :: linorder,'a :: poly_carrier)poly \<Rightarrow> bool"
   where "check_poly_weak_mono_and_pos discrete p \<equiv> 
             if discrete then list_all (\<lambda> v. check_poly_weak_mono_discrete p v) (poly_vars_list p) \<and> eval_poly (\<lambda> w. 0) p \<ge>  0
                         else check_poly_weak_mono_all p"
 
-definition check_poly_weak_anti_mono_discrete :: "('v,'a :: poly_carrier)poly \<Rightarrow> 'v \<Rightarrow> bool"
+definition check_poly_weak_anti_mono_discrete :: "('v :: linorder,'a :: poly_carrier)poly \<Rightarrow> 'v \<Rightarrow> bool"
   where "check_poly_weak_anti_mono_discrete p v \<equiv> check_poly_ge p (poly_subst (\<lambda> w. poly_of (if w = v then PSum [PNum 1, PVar v] else PVar w)) p)"
 
 context poly_order_carrier
 begin
 
 lemma check_poly_weak_mono_discrete: 
-  fixes v :: 'v and p :: "('v,'a)poly"
+  fixes v :: "'v :: linorder" and p :: "('v,'a)poly"
   assumes discrete and check: "check_poly_weak_mono_discrete p v"
   shows "poly_weak_mono p v"
 unfolding poly_weak_mono_def 
@@ -1532,7 +1541,7 @@ proof (intro allI impI)
 qed
 
 lemma check_poly_weak_anti_mono_discrete: 
-  fixes v :: 'v and p :: "('v,'a)poly"
+  fixes v :: "'v :: linorder" and p :: "('v,'a)poly"
   assumes discrete and check: "check_poly_weak_anti_mono_discrete p v"
   shows "poly_weak_anti_mono p v"
 unfolding poly_weak_anti_mono_def 
@@ -1614,7 +1623,7 @@ proof (intro allI impI)
 qed
 
 lemma check_poly_weak_mono_and_pos: 
-  fixes p :: "('v,'a)poly"
+  fixes p :: "('v :: linorder,'a)poly"
   assumes "check_poly_weak_mono_and_pos discrete p"
   shows "poly_weak_mono_all p \<and> (p \<ge>p zero_poly)"
 proof (cases discrete)
@@ -1645,13 +1654,10 @@ qed
 
 end
 
-lemma monom_vars_eval_monom: "\<lbrakk>\<And> x. x \<in> monom_vars m \<Longrightarrow> f x = g x\<rbrakk> \<Longrightarrow> eval_monom f m = eval_monom g m"
-  by (induct m, auto)
-
-definition check_poly_weak_mono :: "('v,'a :: ordered_semiring_0)poly \<Rightarrow> 'v \<Rightarrow> bool"
+definition check_poly_weak_mono :: "('v :: linorder,'a :: ordered_semiring_0)poly \<Rightarrow> 'v \<Rightarrow> bool"
   where "check_poly_weak_mono p v \<equiv> list_all (\<lambda> (m,c). c \<ge> 0 \<or> v \<notin> monom_vars m) p"
 
-lemma check_poly_weak_mono: fixes p :: "('v,'a :: poly_carrier)poly"
+lemma check_poly_weak_mono: fixes p :: "('v :: linorder,'a :: poly_carrier)poly"
   assumes "check_poly_weak_mono p v" shows  "poly_weak_mono p v"
 unfolding poly_weak_mono_def
 proof (intro allI impI)
@@ -1664,8 +1670,6 @@ proof (intro allI impI)
   from assms have "\<And> m c. (m,c) \<in> set p \<Longrightarrow> c \<ge> 0 \<or> v \<notin> monom_vars m" unfolding check_poly_weak_mono_def by (auto simp: list_all_iff)
   thus "eval_poly f p \<ge> eval_poly g p"
   proof (induct p)
-    case Nil thus ?case by (simp add: ge_refl)
-  next
     case (Cons mc p)
     hence IH: "eval_poly f p \<ge> eval_poly g p" by auto
     obtain m c where mc: "mc = (m,c)" by force
@@ -1683,25 +1687,25 @@ proof (intro allI impI)
       next
         assume v: "v \<notin> monom_vars m"
         have "eval_monom f m = eval_monom g m"
-          by (rule monom_vars_eval_monom, insert fg v, auto)
+          by (rule monom_vars_eval_monom, insert fg v, fast)
         thus ?thesis by (simp add: ge_refl)        
       qed
     qed
-  qed
+  qed (simp add: ge_refl)
 qed
 
-definition check_poly_weak_mono_smart :: "bool \<Rightarrow> ('v,'a :: poly_carrier)poly \<Rightarrow> 'v \<Rightarrow> bool"
+definition check_poly_weak_mono_smart :: "bool \<Rightarrow> ('v :: linorder,'a :: poly_carrier)poly \<Rightarrow> 'v \<Rightarrow> bool"
   where "check_poly_weak_mono_smart discrete \<equiv> if discrete then check_poly_weak_mono_discrete else check_poly_weak_mono"
 
-lemma (in poly_order_carrier) check_poly_weak_mono_smart: fixes p :: "('v,'a :: poly_carrier)poly"
+lemma (in poly_order_carrier) check_poly_weak_mono_smart: fixes p :: "('v :: linorder,'a :: poly_carrier)poly"
   shows "check_poly_weak_mono_smart discrete p v \<Longrightarrow> poly_weak_mono p v"
   unfolding check_poly_weak_mono_smart_def
   using check_poly_weak_mono check_poly_weak_mono_discrete by (cases discrete, auto)
 
-definition check_poly_weak_anti_mono :: "('v,'a :: ordered_semiring_0)poly \<Rightarrow> 'v \<Rightarrow> bool"
+definition check_poly_weak_anti_mono :: "('v :: linorder,'a :: ordered_semiring_0)poly \<Rightarrow> 'v \<Rightarrow> bool"
   where "check_poly_weak_anti_mono p v \<equiv> list_all (\<lambda> (m,c). 0 \<ge> c \<or> v \<notin> monom_vars m) p"
 
-lemma check_poly_weak_anti_mono: fixes p :: "('v,'a :: poly_carrier)poly"
+lemma check_poly_weak_anti_mono: fixes p :: "('v :: linorder,'a :: poly_carrier)poly"
   assumes "check_poly_weak_anti_mono p v" shows  "poly_weak_anti_mono p v"
 unfolding poly_weak_anti_mono_def
 proof (intro allI impI)
@@ -1733,54 +1737,87 @@ proof (intro allI impI)
       next
         assume v: "v \<notin> monom_vars m"
         have "eval_monom f m = eval_monom g m"
-          by (rule monom_vars_eval_monom, insert fg v, auto)
+          by (rule monom_vars_eval_monom, insert fg v, fast)
         thus ?thesis by (simp add: ge_refl)        
       qed
     qed
   qed
 qed
 
-definition check_poly_weak_anti_mono_smart :: "bool \<Rightarrow> ('v,'a :: poly_carrier)poly \<Rightarrow> 'v \<Rightarrow> bool"
+definition check_poly_weak_anti_mono_smart :: "bool \<Rightarrow> ('v :: linorder,'a :: poly_carrier)poly \<Rightarrow> 'v \<Rightarrow> bool"
   where "check_poly_weak_anti_mono_smart discrete \<equiv> if discrete then check_poly_weak_anti_mono_discrete else check_poly_weak_anti_mono"
 
-lemma (in poly_order_carrier) check_poly_weak_anti_mono_smart: fixes p :: "('v,'a :: poly_carrier)poly"
+lemma (in poly_order_carrier) check_poly_weak_anti_mono_smart: fixes p :: "('v :: linorder,'a :: poly_carrier)poly"
   shows "check_poly_weak_anti_mono_smart discrete p v \<Longrightarrow> poly_weak_anti_mono p v"
   unfolding check_poly_weak_anti_mono_smart_def
   using check_poly_weak_anti_mono[of p v] check_poly_weak_anti_mono_discrete[of p v] 
   by (cases discrete, auto)
 
-definition check_poly_gt :: "('a \<Rightarrow> 'a \<Rightarrow> bool) \<Rightarrow> ('v,'a :: ordered_semiring_0)poly \<Rightarrow> ('v,'a)poly \<Rightarrow> bool"
-where "check_poly_gt gt p q \<equiv> let (a1,p1) = poly_split [] p; (b1,q1) = poly_split [] q in gt a1 b1 \<and> check_poly_ge p1 q1"
+definition check_poly_gt :: "('a \<Rightarrow> 'a \<Rightarrow> bool) \<Rightarrow> ('v :: linorder,'a :: ordered_semiring_0)poly \<Rightarrow> ('v,'a)poly \<Rightarrow> bool"
+where "check_poly_gt gt p q \<equiv> let (a1,p1) = poly_split 1 p; (b1,q1) = poly_split 1 q in gt a1 b1 \<and> check_poly_ge p1 q1"
 
-definition check_monom_strict_mono :: "bool \<Rightarrow> 'v monom \<Rightarrow> 'v \<Rightarrow> bool"
-  where "check_monom_strict_mono pm m v \<equiv> m \<noteq> [] \<and> tl m = [] \<and> fst (hd m) = v \<and> (\<lambda> p. if pm then 1 \<le> p else p = 1) (snd (hd m))"
+fun univariate_power_list :: "'v \<Rightarrow> 'v monom_list \<Rightarrow> nat option" where
+  "univariate_power_list x [(y,n)] = (if x = y then Some n else None)" 
+| "univariate_power_list _ _ = None" 
 
-definition check_poly_strict_mono :: "bool \<Rightarrow> ('v,'a :: poly_carrier)poly \<Rightarrow> 'v \<Rightarrow> bool"
+lemma univariate_power_list: assumes "monom_inv m" "univariate_power_list x m = Some n" 
+  shows "sum_var_list m = (\<lambda> y. if x = y then n else 0)" 
+   "eval_monom_list \<alpha> m = ((\<alpha> x)^n)" 
+   "n \<ge> 1" 
+proof -
+  have m: "m = [(x,n)]" using assms
+    by (induct x m rule: univariate_power_list.induct, auto split: if_splits)
+  show "eval_monom_list \<alpha> m = ((\<alpha> x)^n)" "sum_var_list m = (\<lambda> y. if x = y then n else 0)"
+    "n \<ge> 1" using assms(1)
+    unfolding m monom_inv_def by (auto simp: sum_var_list_def)
+qed
+
+lift_definition univariate_power :: "'v :: linorder \<Rightarrow> 'v monom \<Rightarrow> nat option" 
+  is univariate_power_list .
+
+lemma univariate_power: assumes "univariate_power x m = Some n" 
+  shows "sum_var m = (\<lambda> y. if x = y then n else 0)" 
+   "eval_monom \<alpha> m = ((\<alpha> x)^n)"
+   "n \<ge> 1" 
+  by (atomize(full), insert assms, transfer, auto dest: univariate_power_list)
+
+definition check_monom_strict_mono :: "bool \<Rightarrow> 'v :: linorder monom \<Rightarrow> 'v \<Rightarrow> bool" where
+  "check_monom_strict_mono pm m v \<equiv> case univariate_power v m of
+     Some p \<Rightarrow> pm \<or> p = 1
+   | None \<Rightarrow> False"
+
+definition check_poly_strict_mono :: "bool \<Rightarrow> ('v :: linorder, 'a :: poly_carrier)poly \<Rightarrow> 'v \<Rightarrow> bool"
   where "check_poly_strict_mono pm p v \<equiv> list_ex (\<lambda> (m,c). (c \<ge> 1) \<and> check_monom_strict_mono pm m v) p"
 
-definition check_poly_strict_mono_discrete :: "('a :: poly_carrier \<Rightarrow> 'a \<Rightarrow> bool) \<Rightarrow> ('v,'a)poly \<Rightarrow> 'v \<Rightarrow> bool"
+definition check_poly_strict_mono_discrete :: "('a :: poly_carrier \<Rightarrow> 'a \<Rightarrow> bool) \<Rightarrow> ('v :: linorder,'a)poly \<Rightarrow> 'v \<Rightarrow> bool"
   where "check_poly_strict_mono_discrete gt p v \<equiv> check_poly_gt gt (poly_subst (\<lambda> w. poly_of (if w = v then PSum [PNum 1, PVar v] else PVar w)) p) p "
 
-definition check_poly_strict_mono_smart :: "bool \<Rightarrow> bool \<Rightarrow> ('a :: poly_carrier \<Rightarrow> 'a \<Rightarrow> bool) \<Rightarrow> ('v,'a)poly \<Rightarrow> 'v \<Rightarrow> bool"
+definition check_poly_strict_mono_smart :: "bool \<Rightarrow> bool \<Rightarrow> ('a :: poly_carrier \<Rightarrow> 'a \<Rightarrow> bool) \<Rightarrow> ('v :: linorder,'a)poly \<Rightarrow> 'v \<Rightarrow> bool"
   where "check_poly_strict_mono_smart discrete pm gt p v \<equiv> 
             if discrete then check_poly_strict_mono_discrete gt p v else check_poly_strict_mono pm p v"
 
-
 context poly_order_carrier
 begin
-lemma check_monom_strict_mono: fixes \<alpha> \<beta> :: "('v,'a)assign" and v :: 'v and m :: "'v monom"
+lemma check_monom_strict_mono: fixes \<alpha> \<beta> :: "('v :: linorder,'a)assign" and v :: 'v and m :: "'v monom"
   assumes check: "check_monom_strict_mono power_mono m v"
   and gt: "\<alpha> v \<succ> \<beta> v"
   and ge: "\<beta> v \<ge> 0"
-  shows "eval_monom \<alpha> m \<succ> eval_monom \<beta> m"
-proof (cases power_mono)
-  case False
-  with check have "m = [(v,1)]" unfolding check_monom_strict_mono_def by (cases m, cases "tl m", cases "hd m", auto)
-  with gt show ?thesis by (auto)
-next
-  case True
-  with check obtain n where m: "m = [(v,n)]" and n: "1 \<le> n" unfolding check_monom_strict_mono_def by (cases m, cases "tl m", cases "hd m", auto)
-  from power_mono[OF True gt ge n] m show ?thesis by auto
+shows "eval_monom \<alpha> m \<succ> eval_monom \<beta> m"
+proof -
+  from check[unfolded check_monom_strict_mono_def] obtain n where
+    uni: "univariate_power v m = Some n" and 1: "\<not> power_mono \<Longrightarrow> n = 1" 
+    by (auto split: option.splits)
+  from univariate_power[OF uni] 
+  have n1: "n \<ge> 1" and eval: "eval_monom a m = a v ^ n" for a :: "('v,'a)assign"
+    by auto
+  show ?thesis
+  proof (cases power_mono)
+    case False
+    with gt 1[OF this] show ?thesis unfolding eval by auto
+  next
+    case True
+    from power_mono[OF True gt ge n1] show ?thesis unfolding eval .
+  qed
 qed
 
 lemma check_poly_strict_mono: 
@@ -1840,11 +1877,11 @@ qed
       
 
 lemma check_poly_gt: 
-  fixes p :: "('v,'a)poly"
+  fixes p :: "('v :: linorder,'a)poly"
   assumes "check_poly_gt gt p q" shows "p >p q"
 proof -
-  obtain a1 p1 where p: "poly_split [] p = (a1,p1)" by (cases "poly_split [] p", auto)
-  obtain b1 q1 where q: "poly_split [] q = (b1,q1)" by (cases "poly_split [] q", auto)
+  obtain a1 p1 where p: "poly_split 1 p = (a1,p1)" by force
+  obtain b1 q1 where q: "poly_split 1 q = (b1,q1)" by force
   from p q assms have gt: "a1 \<succ> b1" and ge: "p1 \<ge>p q1" unfolding check_poly_gt_def using check_poly_ge[of p1 q1]  by auto
   show ?thesis
   proof (unfold poly_gt_def, intro impI allI)
@@ -1858,7 +1895,7 @@ proof -
 qed
 
 lemma check_poly_strict_mono_discrete: 
-  fixes v :: 'v and p :: "('v,'a)poly"
+  fixes v :: "'v :: linorder" and p :: "('v,'a)poly"
   assumes discrete and check: "check_poly_strict_mono_discrete gt p v"
   shows "poly_strict_mono p v"
 unfolding poly_strict_mono_def 
